verse rewrite rules

coq/verse/verse.sig
@@ -3,6 +3,8 @@ Exp  : Type
 Op : Type
 nat : Type
 
+list : Functor
+
 opAdd : Op
 opGt  : Op
 opInt : Op
@@ -10,15 +12,67 @@ opInt : Op
 
 Int   : nat -> Val
 Prim  : Op -> Val
-Tuple : Val -> Val
+Tuple : "list"(Val) -> Val
 Lam   : (Val -> Exp) -> Val
 
 Ret   : Val -> Exp
 App   : Val -> Val -> Exp
 Seq   : Exp -> Exp -> Exp
-Unify : Exp -> Exp -> Exp
+Unify : Val -> Exp -> Exp
 Exists : (Val -> Exp) -> Exp
 Or    : Exp -> Exp -> Exp
 Fail  : Exp 
 One   : Exp -> Exp
 All   : Exp -> Exp
+
+exContext : Type
+Xhole : exContext
+Xeqright : Val -> exContext -> Exp -> exContext
+Xseqleft : exContext -> Exp -> exContext
+Xseqright : Exp -> exContext -> exContext
+
+
+-- ValContext : Type
+-- ValListContext : Type
+-- Vhole : ValContext
+-- Vcons : ValListContext -> ValContext 
+-- VXconsleft : ValContext -> "list" (Val) -> ValListContext 
+-- VXconsright : Val -> ValListContext -> ValListContext
+
+
+SC : Type
+SCchoicehole : SC
+SCchoiceleft : SC -> Exp -> SC
+SCchoiceright : Exp -> SC -> SC
+
+scopeContext : Type 
+SXone : SC -> scopeContext
+SXall : SC -> scopeContext
+
+choiceContext : Type
+CXhole : choiceContext
+CXchoiceright : Val -> choiceContext -> Exp -> choiceContext
+CXseqleft: choiceContext -> Exp -> choiceContext
+CXseqright : Exp -> choiceContext -> choiceContext
+CXexists : (Val -> choiceContext) -> choiceContext
+
+ExpCompatContext : Type 
+ValCompatContext : Type
+ValListCompatContext : Type
+EHole : ExpCompatContext -> ExpCompatContext
+ESeq1 : ExpCompatContext -> Exp -> ExpCompatContext
+ESeq2 : Exp -> ExpCompatContext -> ExpCompatContext
+EUnify1 : ValCompatContext -> Exp -> ExpCompatContext
+EUnify2 : Val -> ExpCompatContext -> ExpCompatContext
+EExists : (Val -> ExpCompatContext) -> ExpCompatContext
+EOr1 : ExpCompatContext -> Exp -> ExpCompatContext
+EOr2 : Exp -> ExpCompatContext -> ExpCompatContext
+EOne : ExpCompatContext -> ExpCompatContext
+EAll : ExpCompatContext -> ExpCompatContext
+EApp1 : ValCompatContext -> Val -> ExpCompatContext
+EApp2 : Val -> ValCompatContext -> ExpCompatContext
+ERet  :ValCompatContext -> ExpCompatContext
+VTuple : ValListCompatContext  -> ValCompatContext
+VLam  : (Val -> ExpCompatContext) -> ValCompatContext
+VEcons1 : ValCompatContext -> "list" (Val) -> ValListCompatContext
+VEcons2 : Val -> ValListCompatContext -> ValListCompatContext
