coq/verse/syntax.v
@@ -1,5 +1,8 @@
 Require Export fintype.
 
+
+
+
 Section Op.
 Inductive Op  : Type :=
   | opAdd : Op 
@@ -18,150 +21,125 @@ Proof. congruence. Qed.
 End Op.
 
 Section ValExp.
-Inductive Val (n : nat) : Type :=
-  | var_Val : fin n -> Val n
-  | Int : nat -> Val n
-  | Prim : Op -> Val n
-  | Tuple : list (Val n) -> Val n
-  | Lam : Exp (S n) -> Val n
- with Exp (n : nat) : Type :=
-  | Ret : Val n -> Exp n
-  | App : Val n -> Val n -> Exp n
-  | Seq : Exp n -> Exp  n -> Exp n
-  | Unify : Val n -> Exp  n -> Exp n
-  | Exists : Exp (S n) -> Exp n
-  | Or : Exp  n -> Exp  n -> Exp n
-  | Fail : Exp n
-  | One : Exp n -> Exp n
-  | All : Exp n -> Exp n.
+Inductive Val (nVal : nat) : Type :=
+  | var_Val : (fin) (nVal) -> Val (nVal)
+  | Int : nat   -> Val (nVal)
+  | Prim : Op   -> Val (nVal)
+  | Tuple : list (Val  (nVal)) -> Val (nVal)
+  | Lam : Exp  ((S) nVal) -> Val (nVal)
+ with Exp (nVal : nat) : Type :=
+  | Ret : Val  (nVal) -> Exp (nVal)
+  | App : Val  (nVal) -> Val  (nVal) -> Exp (nVal)
+  | Seq : Exp  (nVal) -> Exp  (nVal) -> Exp (nVal)
+  | Unify : Val  (nVal) -> Exp  (nVal) -> Exp (nVal)
+  | Exists : Exp  ((S) nVal) -> Exp (nVal)
+  | Or : Exp  (nVal) -> Exp  (nVal) -> Exp (nVal)
+  | Fail : Exp (nVal)
+  | One : Exp  (nVal) -> Exp (nVal)
+  | All : Exp  (nVal) -> Exp (nVal).
 
-Lemma congr_Int { m : nat } { s0 : nat   } { t0 : nat   } (H1 : s0 = t0) : Int m s0 = Int m t0 .
+Lemma congr_Int { mVal : nat } { s0 : nat   } { t0 : nat   } (H1 : s0 = t0) : Int (mVal) s0 = Int (mVal) t0 .
 Proof. congruence. Qed.
 
-Lemma congr_Prim { m : nat } { s0 : Op   } { t0 : Op   } (H1 : s0 = t0) : Prim m s0 = Prim m t0 .
+Lemma congr_Prim { mVal : nat } { s0 : Op   } { t0 : Op   } (H1 : s0 = t0) : Prim (mVal) s0 = Prim (mVal) t0 .
 Proof. congruence. Qed.
 
-Lemma congr_Tuple { m : nat } { s0 : list (Val  m) } { t0 : list (Val  m) } (H1 : s0 = t0) : Tuple m s0 = Tuple m t0 .
+Lemma congr_Tuple { mVal : nat } { s0 : list (Val  (mVal)) } { t0 : list (Val  (mVal)) } (H1 : s0 = t0) : Tuple (mVal) s0 = Tuple (mVal) t0 .
 Proof. congruence. Qed.
 
-Lemma congr_Lam { m : nat } { s0 : Exp  (S m) } { t0 : Exp  (S m) } (H1 : s0 = t0) : Lam m s0 = Lam m t0 .
+Lemma congr_Lam { mVal : nat } { s0 : Exp  ((S) mVal) } { t0 : Exp  ((S) mVal) } (H1 : s0 = t0) : Lam (mVal) s0 = Lam (mVal) t0 .
 Proof. congruence. Qed.
 
-Lemma congr_Ret { m : nat } { s0 : Val  m } { t0 : Val  m } (H1 : s0 = t0) : Ret m s0 = Ret m t0 .
+Lemma congr_Ret { mVal : nat } { s0 : Val  (mVal) } { t0 : Val  (mVal) } (H1 : s0 = t0) : Ret (mVal) s0 = Ret (mVal) t0 .
 Proof. congruence. Qed.
 
-Lemma congr_App { m : nat } { s0 : Val  m } { s1 : Val  m } { t0 : Val  m } { t1 : Val  m } (H1 : s0 = t0) (H2 : s1 = t1) : App m s0 s1 = App m t0 t1 .
+Lemma congr_App { mVal : nat } { s0 : Val  (mVal) } { s1 : Val  (mVal) } { t0 : Val  (mVal) } { t1 : Val  (mVal) } (H1 : s0 = t0) (H2 : s1 = t1) : App (mVal) s0 s1 = App (mVal) t0 t1 .
 Proof. congruence. Qed.
 
-Lemma congr_Seq { m : nat } { s0 : Exp  m } { s1 : Exp  m } { t0 : Exp  m } { t1 : Exp  m } (H1 : s0 = t0) (H2 : s1 = t1) : Seq m s0 s1 = Seq m t0 t1 .
+Lemma congr_Seq { mVal : nat } { s0 : Exp  (mVal) } { s1 : Exp  (mVal) } { t0 : Exp  (mVal) } { t1 : Exp  (mVal) } (H1 : s0 = t0) (H2 : s1 = t1) : Seq (mVal) s0 s1 = Seq (mVal) t0 t1 .
 Proof. congruence. Qed.
 
-Lemma congr_Unify { m : nat } { s0 : Val  m } { s1 : Exp  m } { t0 : Val  m } { t1 : Exp  m } (H1 : s0 = t0) (H2 : s1 = t1) : Unify m s0 s1 = Unify m t0 t1 .
+Lemma congr_Unify { mVal : nat } { s0 : Val  (mVal) } { s1 : Exp  (mVal) } { t0 : Val  (mVal) } { t1 : Exp  (mVal) } (H1 : s0 = t0) (H2 : s1 = t1) : Unify (mVal) s0 s1 = Unify (mVal) t0 t1 .
 Proof. congruence. Qed.
 
-Lemma congr_Exists { m : nat } { s0 : Exp  (S m) } { t0 : Exp  (S m) } (H1 : s0 = t0) : Exists m s0 = Exists m t0 .
+Lemma congr_Exists { mVal : nat } { s0 : Exp  ((S) mVal) } { t0 : Exp  ((S) mVal) } (H1 : s0 = t0) : Exists (mVal) s0 = Exists (mVal) t0 .
 Proof. congruence. Qed.
 
-Lemma congr_Or { m : nat } { s0 : Exp  m } { s1 : Exp  m } { t0 : Exp  m } { t1 : Exp  m } (H1 : s0 = t0) (H2 : s1 = t1) : Or m s0 s1 = Or m t0 t1 .
+Lemma congr_Or { mVal : nat } { s0 : Exp  (mVal) } { s1 : Exp  (mVal) } { t0 : Exp  (mVal) } { t1 : Exp  (mVal) } (H1 : s0 = t0) (H2 : s1 = t1) : Or (mVal) s0 s1 = Or (mVal) t0 t1 .
 Proof. congruence. Qed.
 
-Lemma congr_Fail { m : nat } : Fail m = Fail m .
+Lemma congr_Fail { mVal : nat } : Fail (mVal) = Fail (mVal) .
 Proof. congruence. Qed.
 
-Lemma congr_One { m : nat } { s0 : Exp  m } { t0 : Exp  m } (H1 : s0 = t0) : One m s0 = One m t0 .
+Lemma congr_One { mVal : nat } { s0 : Exp  (mVal) } { t0 : Exp  (mVal) } (H1 : s0 = t0) : One (mVal) s0 = One (mVal) t0 .
 Proof. congruence. Qed.
 
-Lemma congr_All { m : nat } { s0 : Exp  m } { t0 : Exp  m } (H1 : s0 = t0) : All m s0 = All m t0 .
+Lemma congr_All { mVal : nat } { s0 : Exp  (mVal) } { t0 : Exp  (mVal) } (H1 : s0 = t0) : All (mVal) s0 = All (mVal) t0 .
 Proof. congruence. Qed.
 
-Lemma congr_nil {A} : (nil : list A) = nil. Proof. reflexivity. Qed.
-
-Lemma congr_cons {A} {x y : A} {xs ys : list A} (H1 : x = y) (H2 : xs = ys) : cons x xs = cons y ys.
-Proof. congruence. Qed.
-
-Definition upRen_Val_Val { m : nat } { n : nat } (xi : fin m -> fin (n)) : fin (S m) -> fin (S (n)) :=
+Definition upRen_Val_Val { m : nat } { n : nat } (xi : (fin) (m) -> (fin) (n)) : (fin) ((S) (m)) -> (fin) ((S) (n)) :=
   (up_ren) xi.
 
-
-Fixpoint ren_Val { m : nat } { n : nat } (xiVal : fin m -> fin n) (s : Val m) : Val n :=
-  let ren_Vals (vs : list (Val m)) := List.map (ren_Val xiVal) vs in
-    match s return Val n with
-    | var_Val (_) s => (var_Val n) (xiVal s)
-    | Int (_) s0 => Int n ((fun x => x) s0)
-    | Prim (_) s0 => Prim n ((fun x => x) s0)
-    | Tuple (_) s0 => Tuple n (ren_Vals s0)
-    | Lam (_) s0 => Lam n ((ren_Exp (upRen_Val_Val xiVal)) s0)
+Fixpoint ren_Val { mVal : nat } { nVal : nat } (xiVal : (fin) (mVal) -> (fin) (nVal)) (s : Val (mVal)) : Val (nVal) :=
+    match s return Val (nVal) with
+    | var_Val (_) s => (var_Val (nVal)) (xiVal s)
+    | Int (_) s0 => Int (nVal) ((fun x => x) s0)
+    | Prim (_) s0 => Prim (nVal) ((fun x => x) s0)
+    | Tuple (_) s0 => Tuple (nVal) ((list_map (ren_Val xiVal)) s0)
+    | Lam (_) s0 => Lam (nVal) ((ren_Exp (upRen_Val_Val xiVal)) s0)
     end
- with ren_Exp { m : nat } { n : nat } (xiVal : fin m -> fin n) (s : Exp m) : Exp n :=
-    match s return Exp n with
-    | Ret (_) s0 => Ret n ((ren_Val xiVal) s0)
-    | App (_) s0 s1 => App n ((ren_Val xiVal) s0) ((ren_Val xiVal) s1)
-    | Seq (_) s0 s1 => Seq n ((ren_Exp xiVal) s0) ((ren_Exp xiVal) s1)
-    | Unify (_) s0 s1 => Unify n ((ren_Val xiVal) s0) ((ren_Exp xiVal) s1)
-    | Exists (_) s0 => Exists n ((ren_Exp (upRen_Val_Val xiVal)) s0)
-    | Or (_) s0 s1 => Or n ((ren_Exp xiVal) s0) ((ren_Exp xiVal) s1)
-    | Fail (_)  => Fail n
-    | One (_) s0 => One n ((ren_Exp xiVal) s0)
-    | All (_) s0 => All n ((ren_Exp xiVal) s0)
+ with ren_Exp { mVal : nat } { nVal : nat } (xiVal : (fin) (mVal) -> (fin) (nVal)) (s : Exp (mVal)) : Exp (nVal) :=
+    match s return Exp (nVal) with
+    | Ret (_) s0 => Ret (nVal) ((ren_Val xiVal) s0)
+    | App (_) s0 s1 => App (nVal) ((ren_Val xiVal) s0) ((ren_Val xiVal) s1)
+    | Seq (_) s0 s1 => Seq (nVal) ((ren_Exp xiVal) s0) ((ren_Exp xiVal) s1)
+    | Unify (_) s0 s1 => Unify (nVal) ((ren_Val xiVal) s0) ((ren_Exp xiVal) s1)
+    | Exists (_) s0 => Exists (nVal) ((ren_Exp (upRen_Val_Val xiVal)) s0)
+    | Or (_) s0 s1 => Or (nVal) ((ren_Exp xiVal) s0) ((ren_Exp xiVal) s1)
+    | Fail (_)  => Fail (nVal)
+    | One (_) s0 => One (nVal) ((ren_Exp xiVal) s0)
+    | All (_) s0 => All (nVal) ((ren_Exp xiVal) s0)
     end.
 
-Definition ren_Vals {m}{n} (xiVal : fin m -> fin n) (vs : list (Val m)) := 
-  List.map (ren_Val xiVal) vs.
+Definition up_Val_Val { m : nat } { nVal : nat } (sigma : (fin) (m) -> Val (nVal)) : (fin) ((S) (m)) -> Val ((S) nVal) :=
+  (scons) ((var_Val ((S) nVal)) (var_zero)) ((funcomp) (ren_Val (shift)) sigma).
 
-Definition up_Val_Val { m : nat } { n : nat } (sigma : fin m -> Val n) : fin (S m) -> Val (S n) :=
-  (scons) ((var_Val (S n)) (var_zero)) ((funcomp) (ren_Val (shift)) sigma).
-
-Fixpoint subst_Val { m : nat } { n : nat } (sigmaVal : fin m -> Val n) (s : Val m) : Val n :=
-  let subst_Vals (vs : list (Val m)) := 
-    List.map (subst_Val sigmaVal) vs in
-    match s return Val n with
+Fixpoint subst_Val { mVal : nat } { nVal : nat } (sigmaVal : (fin) (mVal) -> Val (nVal)) (s : Val (mVal)) : Val (nVal) :=
+    match s return Val (nVal) with
     | var_Val (_) s => sigmaVal s
-    | Int (_) s0 => Int n ((fun x => x) s0)
-    | Prim (_) s0 => Prim n ((fun x => x) s0)
-    | Tuple (_) s0 => Tuple n (subst_Vals s0)
-    | Lam (_) s0 => Lam n ((subst_Exp (up_Val_Val sigmaVal)) s0)
+    | Int (_) s0 => Int (nVal) ((fun x => x) s0)
+    | Prim (_) s0 => Prim (nVal) ((fun x => x) s0)
+    | Tuple (_) s0 => Tuple (nVal) ((list_map (subst_Val sigmaVal)) s0)
+    | Lam (_) s0 => Lam (nVal) ((subst_Exp (up_Val_Val sigmaVal)) s0)
     end
- with subst_Exp { m : nat } { n : nat } (sigmaVal : fin m -> Val n) (s : Exp m) : Exp n :=
-    match s return Exp n with
-    | Ret (_) s0 => Ret n ((subst_Val sigmaVal) s0)
-    | App (_) s0 s1 => App n ((subst_Val sigmaVal) s0) ((subst_Val sigmaVal) s1)
-    | Seq (_) s0 s1 => Seq n ((subst_Exp sigmaVal) s0) ((subst_Exp sigmaVal) s1)
-    | Unify (_) s0 s1 => Unify n ((subst_Val sigmaVal) s0) ((subst_Exp sigmaVal) s1)
-    | Exists (_) s0 => Exists n ((subst_Exp (up_Val_Val sigmaVal)) s0)
-    | Or (_) s0 s1 => Or n ((subst_Exp sigmaVal) s0) ((subst_Exp sigmaVal) s1)
-    | Fail (_)  => Fail n
-    | One (_) s0 => One n ((subst_Exp sigmaVal) s0)
-    | All (_) s0 => All n ((subst_Exp sigmaVal) s0)
+ with subst_Exp { mVal : nat } { nVal : nat } (sigmaVal : (fin) (mVal) -> Val (nVal)) (s : Exp (mVal)) : Exp (nVal) :=
+    match s return Exp (nVal) with
+    | Ret (_) s0 => Ret (nVal) ((subst_Val sigmaVal) s0)
+    | App (_) s0 s1 => App (nVal) ((subst_Val sigmaVal) s0) ((subst_Val sigmaVal) s1)
+    | Seq (_) s0 s1 => Seq (nVal) ((subst_Exp sigmaVal) s0) ((subst_Exp sigmaVal) s1)
+    | Unify (_) s0 s1 => Unify (nVal) ((subst_Val sigmaVal) s0) ((subst_Exp sigmaVal) s1)
+    | Exists (_) s0 => Exists (nVal) ((subst_Exp (up_Val_Val sigmaVal)) s0)
+    | Or (_) s0 s1 => Or (nVal) ((subst_Exp sigmaVal) s0) ((subst_Exp sigmaVal) s1)
+    | Fail (_)  => Fail (nVal)
+    | One (_) s0 => One (nVal) ((subst_Exp sigmaVal) s0)
+    | All (_) s0 => All (nVal) ((subst_Exp sigmaVal) s0)
     end.
 
-Definition subst_Vals { m : nat } { n : nat } (sigmaVal : fin m -> Val n) 
-  (vs : list (Val m)) : list (Val n) := List.map (subst_Val sigmaVal) vs.
-
-Definition upId_Val_Val { m : nat } (sigma : fin m -> Val m) (Eq : forall x, sigma x = (var_Val m) x) : forall x, (up_Val_Val sigma) x = (var_Val (S m)) x :=
+Definition upId_Val_Val { mVal : nat } (sigma : (fin) (mVal) -> Val (mVal)) (Eq : forall x, sigma x = (var_Val (mVal)) x) : forall x, (up_Val_Val sigma) x = (var_Val ((S) mVal)) x :=
   fun n => match n with
   | Some fin_n => (ap) (ren_Val (shift)) (Eq fin_n)
   | None  => eq_refl
   end.
 
-
-Definition idSubst_nil { m } : 
-  forall (sigmaVal : fin m -> Val m), subst_Vals sigmaVal nil = nil := fun s => eq_refl.
-
-
-Fixpoint idSubst_Val { m : nat } (sigmaVal : fin m -> Val m) (EqVal : forall x, sigmaVal x = (var_Val m) x) (s : Val m) : subst_Val sigmaVal s = s :=
-  let fix idSubst_Vals (vs : list (Val m)) : subst_Vals sigmaVal vs = vs := 
-         match vs with
-         | nil => idSubst_nil sigmaVal
-         | cons v vs' => congr_cons (idSubst_Val sigmaVal EqVal v) (idSubst_Vals vs')
-         end in
+Fixpoint idSubst_Val { mVal : nat } (sigmaVal : (fin) (mVal) -> Val (mVal)) (EqVal : forall x, sigmaVal x = (var_Val (mVal)) x) (s : Val (mVal)) : subst_Val sigmaVal s = s :=
     match s return subst_Val sigmaVal s = s with
     | var_Val (_) s => EqVal s
     | Int (_) s0 => congr_Int ((fun x => (eq_refl) x) s0)
     | Prim (_) s0 => congr_Prim ((fun x => (eq_refl) x) s0)
-    | Tuple (_) s0 => congr_Tuple (idSubst_Vals s0)
+    | Tuple (_) s0 => congr_Tuple ((list_id (idSubst_Val sigmaVal EqVal)) s0)
     | Lam (_) s0 => congr_Lam ((idSubst_Exp (up_Val_Val sigmaVal) (upId_Val_Val (_) EqVal)) s0)
     end
- with idSubst_Exp { m : nat } (sigmaVal : fin m -> Val m) (EqVal : forall x, sigmaVal x = (var_Val m) x) (s : Exp m) : subst_Exp sigmaVal s = s :=
+ with idSubst_Exp { mVal : nat } (sigmaVal : (fin) (mVal) -> Val (mVal)) (EqVal : forall x, sigmaVal x = (var_Val (mVal)) x) (s : Exp (mVal)) : subst_Exp sigmaVal s = s :=
     match s return subst_Exp sigmaVal s = s with
     | Ret (_) s0 => congr_Ret ((idSubst_Val sigmaVal EqVal) s0)
     | App (_) s0 s1 => congr_App ((idSubst_Val sigmaVal EqVal) s0) ((idSubst_Val sigmaVal EqVal) s1)
@@ -174,26 +152,21 @@ Fixpoint idSubst_Val { m : nat } (sigmaVal : fin m -> Val m) (EqVal : forall x, 
     | All (_) s0 => congr_All ((idSubst_Exp sigmaVal EqVal) s0)
     end.
 
-Definition upExtRen_Val_Val { m : nat } { n : nat } (xi : fin m -> fin (n)) (zeta : fin m -> fin (n)) (Eq : forall x, xi x = zeta x) : forall x, (upRen_Val_Val xi) x = (upRen_Val_Val zeta) x :=
+Definition upExtRen_Val_Val { m : nat } { n : nat } (xi : (fin) (m) -> (fin) (n)) (zeta : (fin) (m) -> (fin) (n)) (Eq : forall x, xi x = zeta x) : forall x, (upRen_Val_Val xi) x = (upRen_Val_Val zeta) x :=
   fun n => match n with
   | Some fin_n => (ap) (shift) (Eq fin_n)
   | None  => eq_refl
   end.
 
-Fixpoint extRen_Val { m : nat } { n : nat } (xiVal : fin m -> fin n) (zetaVal : fin m -> fin n) (EqVal : forall x, xiVal x = zetaVal x) (s : Val m) : ren_Val xiVal s = ren_Val zetaVal s :=
-    let fix extRen_Vals (vs : list (Val m)) := 
-      match vs return ren_Vals xiVal vs = ren_Vals zetaVal vs with 
-      | nil => eq_refl
-      | cons v vs' => congr_cons (extRen_Val xiVal zetaVal EqVal v) (extRen_Vals vs')
-        end in
+Fixpoint extRen_Val { mVal : nat } { nVal : nat } (xiVal : (fin) (mVal) -> (fin) (nVal)) (zetaVal : (fin) (mVal) -> (fin) (nVal)) (EqVal : forall x, xiVal x = zetaVal x) (s : Val (mVal)) : ren_Val xiVal s = ren_Val zetaVal s :=
     match s return ren_Val xiVal s = ren_Val zetaVal s with
-    | var_Val (_) s => (ap) (var_Val n) (EqVal s)
+    | var_Val (_) s => (ap) (var_Val (nVal)) (EqVal s)
     | Int (_) s0 => congr_Int ((fun x => (eq_refl) x) s0)
     | Prim (_) s0 => congr_Prim ((fun x => (eq_refl) x) s0)
-    | Tuple (_) s0 => congr_Tuple (extRen_Vals s0)
+    | Tuple (_) s0 => congr_Tuple ((list_ext (extRen_Val xiVal zetaVal EqVal)) s0)
     | Lam (_) s0 => congr_Lam ((extRen_Exp (upRen_Val_Val xiVal) (upRen_Val_Val zetaVal) (upExtRen_Val_Val (_) (_) EqVal)) s0)
     end
- with extRen_Exp { m : nat } { n : nat } (xiVal : fin m -> fin n) (zetaVal : fin m -> fin n) (EqVal : forall x, xiVal x = zetaVal x) (s : Exp m) : ren_Exp xiVal s = ren_Exp zetaVal s :=
+ with extRen_Exp { mVal : nat } { nVal : nat } (xiVal : (fin) (mVal) -> (fin) (nVal)) (zetaVal : (fin) (mVal) -> (fin) (nVal)) (EqVal : forall x, xiVal x = zetaVal x) (s : Exp (mVal)) : ren_Exp xiVal s = ren_Exp zetaVal s :=
     match s return ren_Exp xiVal s = ren_Exp zetaVal s with
     | Ret (_) s0 => congr_Ret ((extRen_Val xiVal zetaVal EqVal) s0)
     | App (_) s0 s1 => congr_App ((extRen_Val xiVal zetaVal EqVal) s0) ((extRen_Val xiVal zetaVal EqVal) s1)
@@ -206,26 +179,21 @@ Fixpoint extRen_Val { m : nat } { n : nat } (xiVal : fin m -> fin n) (zetaVal : 
     | All (_) s0 => congr_All ((extRen_Exp xiVal zetaVal EqVal) s0)
     end.
 
-Definition upExt_Val_Val { m : nat } { n : nat } (sigma : fin m -> Val n) (tau : fin m -> Val n) (Eq : forall x, sigma x = tau x) : forall x, (up_Val_Val sigma) x = (up_Val_Val tau) x :=
+Definition upExt_Val_Val { m : nat } { nVal : nat } (sigma : (fin) (m) -> Val (nVal)) (tau : (fin) (m) -> Val (nVal)) (Eq : forall x, sigma x = tau x) : forall x, (up_Val_Val sigma) x = (up_Val_Val tau) x :=
   fun n => match n with
   | Some fin_n => (ap) (ren_Val (shift)) (Eq fin_n)
   | None  => eq_refl
   end.
 
-Fixpoint ext_Val { m : nat } { n : nat } (sigmaVal : fin m -> Val n) (tauVal : fin m -> Val n) (EqVal : forall x, sigmaVal x = tauVal x) (s : Val m) : subst_Val sigmaVal s = subst_Val tauVal s :=
-    let fix ext_Vals (vs : list (Val m)) :=       
-      match vs return subst_Vals sigmaVal vs = subst_Vals tauVal vs with  
-      | nil => eq_refl
-      | cons v vs' => congr_cons (ext_Val sigmaVal tauVal EqVal v) (ext_Vals vs')
-      end in
+Fixpoint ext_Val { mVal : nat } { nVal : nat } (sigmaVal : (fin) (mVal) -> Val (nVal)) (tauVal : (fin) (mVal) -> Val (nVal)) (EqVal : forall x, sigmaVal x = tauVal x) (s : Val (mVal)) : subst_Val sigmaVal s = subst_Val tauVal s :=
     match s return subst_Val sigmaVal s = subst_Val tauVal s with
     | var_Val (_) s => EqVal s
     | Int (_) s0 => congr_Int ((fun x => (eq_refl) x) s0)
     | Prim (_) s0 => congr_Prim ((fun x => (eq_refl) x) s0)
-    | Tuple (_) s0 => congr_Tuple (ext_Vals s0)
+    | Tuple (_) s0 => congr_Tuple ((list_ext (ext_Val sigmaVal tauVal EqVal)) s0)
     | Lam (_) s0 => congr_Lam ((ext_Exp (up_Val_Val sigmaVal) (up_Val_Val tauVal) (upExt_Val_Val (_) (_) EqVal)) s0)
     end
- with ext_Exp { m : nat } { n : nat } (sigmaVal : fin m -> Val n) (tauVal : fin m -> Val n) (EqVal : forall x, sigmaVal x = tauVal x) (s : Exp m) : subst_Exp sigmaVal s = subst_Exp tauVal s :=
+ with ext_Exp { mVal : nat } { nVal : nat } (sigmaVal : (fin) (mVal) -> Val (nVal)) (tauVal : (fin) (mVal) -> Val (nVal)) (EqVal : forall x, sigmaVal x = tauVal x) (s : Exp (mVal)) : subst_Exp sigmaVal s = subst_Exp tauVal s :=
     match s return subst_Exp sigmaVal s = subst_Exp tauVal s with
     | Ret (_) s0 => congr_Ret ((ext_Val sigmaVal tauVal EqVal) s0)
     | App (_) s0 s1 => congr_App ((ext_Val sigmaVal tauVal EqVal) s0) ((ext_Val sigmaVal tauVal EqVal) s1)
@@ -238,24 +206,18 @@ Fixpoint ext_Val { m : nat } { n : nat } (sigmaVal : fin m -> Val n) (tauVal : f
     | All (_) s0 => congr_All ((ext_Exp sigmaVal tauVal EqVal) s0)
     end.
 
-Definition up_ren_ren_Val_Val { k : nat } { l : nat } { m : nat } (xi : fin (k) -> fin (l)) (tau : fin (l) -> fin m) (theta : fin (k) -> fin m) (Eq : forall x, ((funcomp) tau xi) x = theta x) : forall x, ((funcomp) (upRen_Val_Val tau) (upRen_Val_Val xi)) x = (upRen_Val_Val theta) x :=
+Definition up_ren_ren_Val_Val { k : nat } { l : nat } { m : nat } (xi : (fin) (k) -> (fin) (l)) (tau : (fin) (l) -> (fin) (m)) (theta : (fin) (k) -> (fin) (m)) (Eq : forall x, ((funcomp) tau xi) x = theta x) : forall x, ((funcomp) (upRen_Val_Val tau) (upRen_Val_Val xi)) x = (upRen_Val_Val theta) x :=
   up_ren_ren xi tau theta Eq.
 
-Fixpoint compRenRen_Val { kVal : nat } { lVal : nat } { m : nat } (xiVal : fin m -> fin (kVal)) (zetaVal : fin (kVal) -> fin (lVal)) (rhoVal : fin m -> fin (lVal)) (EqVal : forall x, ((funcomp) zetaVal xiVal) x = rhoVal x) (s : Val m) : ren_Val zetaVal (ren_Val xiVal s) = ren_Val rhoVal s :=
-  let fix compRenRen_Vals (vs : list (Val m)) := 
-    match vs return ren_Vals zetaVal (ren_Vals xiVal vs) = ren_Vals rhoVal vs with 
-    | nil => eq_refl
-    | cons v vs' => congr_cons (compRenRen_Val xiVal zetaVal rhoVal EqVal v)
-                              (compRenRen_Vals vs')
-    end in
+Fixpoint compRenRen_Val { kVal : nat } { lVal : nat } { mVal : nat } (xiVal : (fin) (mVal) -> (fin) (kVal)) (zetaVal : (fin) (kVal) -> (fin) (lVal)) (rhoVal : (fin) (mVal) -> (fin) (lVal)) (EqVal : forall x, ((funcomp) zetaVal xiVal) x = rhoVal x) (s : Val (mVal)) : ren_Val zetaVal (ren_Val xiVal s) = ren_Val rhoVal s :=
     match s return ren_Val zetaVal (ren_Val xiVal s) = ren_Val rhoVal s with
     | var_Val (_) s => (ap) (var_Val (lVal)) (EqVal s)
     | Int (_) s0 => congr_Int ((fun x => (eq_refl) x) s0)
     | Prim (_) s0 => congr_Prim ((fun x => (eq_refl) x) s0)
-    | Tuple (_) s0 => congr_Tuple (compRenRen_Vals s0)
+    | Tuple (_) s0 => congr_Tuple ((list_comp (compRenRen_Val xiVal zetaVal rhoVal EqVal)) s0)
     | Lam (_) s0 => congr_Lam ((compRenRen_Exp (upRen_Val_Val xiVal) (upRen_Val_Val zetaVal) (upRen_Val_Val rhoVal) (up_ren_ren (_) (_) (_) EqVal)) s0)
     end
- with compRenRen_Exp { kVal : nat } { lVal : nat } { m : nat } (xiVal : fin m -> fin (kVal)) (zetaVal : fin (kVal) -> fin (lVal)) (rhoVal : fin m -> fin (lVal)) (EqVal : forall x, ((funcomp) zetaVal xiVal) x = rhoVal x) (s : Exp m) : ren_Exp zetaVal (ren_Exp xiVal s) = ren_Exp rhoVal s :=
+ with compRenRen_Exp { kVal : nat } { lVal : nat } { mVal : nat } (xiVal : (fin) (mVal) -> (fin) (kVal)) (zetaVal : (fin) (kVal) -> (fin) (lVal)) (rhoVal : (fin) (mVal) -> (fin) (lVal)) (EqVal : forall x, ((funcomp) zetaVal xiVal) x = rhoVal x) (s : Exp (mVal)) : ren_Exp zetaVal (ren_Exp xiVal s) = ren_Exp rhoVal s :=
     match s return ren_Exp zetaVal (ren_Exp xiVal s) = ren_Exp rhoVal s with
     | Ret (_) s0 => congr_Ret ((compRenRen_Val xiVal zetaVal rhoVal EqVal) s0)
     | App (_) s0 s1 => congr_App ((compRenRen_Val xiVal zetaVal rhoVal EqVal) s0) ((compRenRen_Val xiVal zetaVal rhoVal EqVal) s1)
@@ -268,27 +230,21 @@ Fixpoint compRenRen_Val { kVal : nat } { lVal : nat } { m : nat } (xiVal : fin m
     | All (_) s0 => congr_All ((compRenRen_Exp xiVal zetaVal rhoVal EqVal) s0)
     end.
 
-Definition up_ren_subst_Val_Val { k : nat } { l : nat } { m : nat } (xi : fin (k) -> fin (l)) (tau : fin (l) -> Val m) (theta : fin (k) -> Val m) (Eq : forall x, ((funcomp) tau xi) x = theta x) : forall x, ((funcomp) (up_Val_Val tau) (upRen_Val_Val xi)) x = (up_Val_Val theta) x :=
+Definition up_ren_subst_Val_Val { k : nat } { l : nat } { mVal : nat } (xi : (fin) (k) -> (fin) (l)) (tau : (fin) (l) -> Val (mVal)) (theta : (fin) (k) -> Val (mVal)) (Eq : forall x, ((funcomp) tau xi) x = theta x) : forall x, ((funcomp) (up_Val_Val tau) (upRen_Val_Val xi)) x = (up_Val_Val theta) x :=
   fun n => match n with
   | Some fin_n => (ap) (ren_Val (shift)) (Eq fin_n)
   | None  => eq_refl
   end.
 
-Fixpoint compRenSubst_Val { kVal : nat } { lVal : nat } { m : nat } (xiVal : fin m -> fin (kVal)) (tauVal : fin (kVal) -> Val (lVal)) (thetaVal : fin m -> Val (lVal)) (EqVal : forall x, ((funcomp) tauVal xiVal) x = thetaVal x) (s : Val m) : subst_Val tauVal (ren_Val xiVal s) = subst_Val thetaVal s :=
-  let fix compRenSubst_Vals (vs : list (Val m)) := 
-    match vs return subst_Vals tauVal (ren_Vals xiVal vs) = subst_Vals thetaVal vs with
-    | nil => eq_refl
-    | cons v vs' => congr_cons (compRenSubst_Val xiVal tauVal thetaVal EqVal v)
-                              (compRenSubst_Vals vs')
-    end in
+Fixpoint compRenSubst_Val { kVal : nat } { lVal : nat } { mVal : nat } (xiVal : (fin) (mVal) -> (fin) (kVal)) (tauVal : (fin) (kVal) -> Val (lVal)) (thetaVal : (fin) (mVal) -> Val (lVal)) (EqVal : forall x, ((funcomp) tauVal xiVal) x = thetaVal x) (s : Val (mVal)) : subst_Val tauVal (ren_Val xiVal s) = subst_Val thetaVal s :=
     match s return subst_Val tauVal (ren_Val xiVal s) = subst_Val thetaVal s with
     | var_Val (_) s => EqVal s
     | Int (_) s0 => congr_Int ((fun x => (eq_refl) x) s0)
     | Prim (_) s0 => congr_Prim ((fun x => (eq_refl) x) s0)
-    | Tuple (_) s0 => congr_Tuple (compRenSubst_Vals s0)
+    | Tuple (_) s0 => congr_Tuple ((list_comp (compRenSubst_Val xiVal tauVal thetaVal EqVal)) s0)
     | Lam (_) s0 => congr_Lam ((compRenSubst_Exp (upRen_Val_Val xiVal) (up_Val_Val tauVal) (up_Val_Val thetaVal) (up_ren_subst_Val_Val (_) (_) (_) EqVal)) s0)
     end
- with compRenSubst_Exp { kVal : nat } { lVal : nat } { m : nat } (xiVal : fin m -> fin (kVal)) (tauVal : fin (kVal) -> Val (lVal)) (thetaVal : fin m -> Val (lVal)) (EqVal : forall x, ((funcomp) tauVal xiVal) x = thetaVal x) (s : Exp m) : subst_Exp tauVal (ren_Exp xiVal s) = subst_Exp thetaVal s :=
+ with compRenSubst_Exp { kVal : nat } { lVal : nat } { mVal : nat } (xiVal : (fin) (mVal) -> (fin) (kVal)) (tauVal : (fin) (kVal) -> Val (lVal)) (thetaVal : (fin) (mVal) -> Val (lVal)) (EqVal : forall x, ((funcomp) tauVal xiVal) x = thetaVal x) (s : Exp (mVal)) : subst_Exp tauVal (ren_Exp xiVal s) = subst_Exp thetaVal s :=
     match s return subst_Exp tauVal (ren_Exp xiVal s) = subst_Exp thetaVal s with
     | Ret (_) s0 => congr_Ret ((compRenSubst_Val xiVal tauVal thetaVal EqVal) s0)
     | App (_) s0 s1 => congr_App ((compRenSubst_Val xiVal tauVal thetaVal EqVal) s0) ((compRenSubst_Val xiVal tauVal thetaVal EqVal) s1)
@@ -301,28 +257,21 @@ Fixpoint compRenSubst_Val { kVal : nat } { lVal : nat } { m : nat } (xiVal : fin
     | All (_) s0 => congr_All ((compRenSubst_Exp xiVal tauVal thetaVal EqVal) s0)
     end.
 
-Definition up_subst_ren_Val_Val { k : nat } { lVal : nat } { m : nat } (sigma : fin (k) -> Val (lVal)) (zetaVal : fin (lVal) -> fin m) (theta : fin (k) -> Val m) (Eq : forall x, ((funcomp) (ren_Val zetaVal) sigma) x = theta x) : forall x, ((funcomp) (ren_Val (upRen_Val_Val zetaVal)) (up_Val_Val sigma)) x = (up_Val_Val theta) x :=
+Definition up_subst_ren_Val_Val { k : nat } { lVal : nat } { mVal : nat } (sigma : (fin) (k) -> Val (lVal)) (zetaVal : (fin) (lVal) -> (fin) (mVal)) (theta : (fin) (k) -> Val (mVal)) (Eq : forall x, ((funcomp) (ren_Val zetaVal) sigma) x = theta x) : forall x, ((funcomp) (ren_Val (upRen_Val_Val zetaVal)) (up_Val_Val sigma)) x = (up_Val_Val theta) x :=
   fun n => match n with
   | Some fin_n => (eq_trans) (compRenRen_Val (shift) (upRen_Val_Val zetaVal) ((funcomp) (shift) zetaVal) (fun x => eq_refl) (sigma fin_n)) ((eq_trans) ((eq_sym) (compRenRen_Val zetaVal (shift) ((funcomp) (shift) zetaVal) (fun x => eq_refl) (sigma fin_n))) ((ap) (ren_Val (shift)) (Eq fin_n)))
   | None  => eq_refl
   end.
 
-Fixpoint compSubstRen_Val { kVal : nat } { lVal : nat } { m : nat } (sigmaVal : fin m -> Val (kVal)) (zetaVal : fin (kVal) -> fin (lVal)) (thetaVal : fin m -> Val (lVal)) (EqVal : forall x, ((funcomp) (ren_Val zetaVal) sigmaVal) x = thetaVal x) (s : Val m) : ren_Val zetaVal (subst_Val sigmaVal s) = subst_Val thetaVal s :=
-  let fix compSubstRen_Vals (vs : list( Val m)) := 
-    match vs return ren_Vals zetaVal (subst_Vals sigmaVal vs) = subst_Vals thetaVal vs with
-    | nil => eq_refl
-    | cons v vs' => congr_cons (compSubstRen_Val sigmaVal zetaVal thetaVal EqVal v)
-                              (compSubstRen_Vals vs')
-    end in
-    match s return
-          ren_Val zetaVal (subst_Val sigmaVal s) = subst_Val thetaVal s with
+Fixpoint compSubstRen_Val { kVal : nat } { lVal : nat } { mVal : nat } (sigmaVal : (fin) (mVal) -> Val (kVal)) (zetaVal : (fin) (kVal) -> (fin) (lVal)) (thetaVal : (fin) (mVal) -> Val (lVal)) (EqVal : forall x, ((funcomp) (ren_Val zetaVal) sigmaVal) x = thetaVal x) (s : Val (mVal)) : ren_Val zetaVal (subst_Val sigmaVal s) = subst_Val thetaVal s :=
+    match s return ren_Val zetaVal (subst_Val sigmaVal s) = subst_Val thetaVal s with
     | var_Val (_) s => EqVal s
     | Int (_) s0 => congr_Int ((fun x => (eq_refl) x) s0)
     | Prim (_) s0 => congr_Prim ((fun x => (eq_refl) x) s0)
-    | Tuple (_) s0 => congr_Tuple (compSubstRen_Vals s0)
+    | Tuple (_) s0 => congr_Tuple ((list_comp (compSubstRen_Val sigmaVal zetaVal thetaVal EqVal)) s0)
     | Lam (_) s0 => congr_Lam ((compSubstRen_Exp (up_Val_Val sigmaVal) (upRen_Val_Val zetaVal) (up_Val_Val thetaVal) (up_subst_ren_Val_Val (_) (_) (_) EqVal)) s0)
     end
- with compSubstRen_Exp { kVal : nat } { lVal : nat } { m : nat } (sigmaVal : fin m -> Val (kVal)) (zetaVal : fin (kVal) -> fin (lVal)) (thetaVal : fin m -> Val (lVal)) (EqVal : forall x, ((funcomp) (ren_Val zetaVal) sigmaVal) x = thetaVal x) (s : Exp m) : ren_Exp zetaVal (subst_Exp sigmaVal s) = subst_Exp thetaVal s :=
+ with compSubstRen_Exp { kVal : nat } { lVal : nat } { mVal : nat } (sigmaVal : (fin) (mVal) -> Val (kVal)) (zetaVal : (fin) (kVal) -> (fin) (lVal)) (thetaVal : (fin) (mVal) -> Val (lVal)) (EqVal : forall x, ((funcomp) (ren_Val zetaVal) sigmaVal) x = thetaVal x) (s : Exp (mVal)) : ren_Exp zetaVal (subst_Exp sigmaVal s) = subst_Exp thetaVal s :=
     match s return ren_Exp zetaVal (subst_Exp sigmaVal s) = subst_Exp thetaVal s with
     | Ret (_) s0 => congr_Ret ((compSubstRen_Val sigmaVal zetaVal thetaVal EqVal) s0)
     | App (_) s0 s1 => congr_App ((compSubstRen_Val sigmaVal zetaVal thetaVal EqVal) s0) ((compSubstRen_Val sigmaVal zetaVal thetaVal EqVal) s1)
@@ -335,27 +284,21 @@ Fixpoint compSubstRen_Val { kVal : nat } { lVal : nat } { m : nat } (sigmaVal : 
     | All (_) s0 => congr_All ((compSubstRen_Exp sigmaVal zetaVal thetaVal EqVal) s0)
     end.
 
-Definition up_subst_subst_Val_Val { k : nat } { lVal : nat } { m : nat } (sigma : fin (k) -> Val (lVal)) (tauVal : fin (lVal) -> Val m) (theta : fin (k) -> Val m) (Eq : forall x, ((funcomp) (subst_Val tauVal) sigma) x = theta x) : forall x, ((funcomp) (subst_Val (up_Val_Val tauVal)) (up_Val_Val sigma)) x = (up_Val_Val theta) x :=
+Definition up_subst_subst_Val_Val { k : nat } { lVal : nat } { mVal : nat } (sigma : (fin) (k) -> Val (lVal)) (tauVal : (fin) (lVal) -> Val (mVal)) (theta : (fin) (k) -> Val (mVal)) (Eq : forall x, ((funcomp) (subst_Val tauVal) sigma) x = theta x) : forall x, ((funcomp) (subst_Val (up_Val_Val tauVal)) (up_Val_Val sigma)) x = (up_Val_Val theta) x :=
   fun n => match n with
   | Some fin_n => (eq_trans) (compRenSubst_Val (shift) (up_Val_Val tauVal) ((funcomp) (up_Val_Val tauVal) (shift)) (fun x => eq_refl) (sigma fin_n)) ((eq_trans) ((eq_sym) (compSubstRen_Val tauVal (shift) ((funcomp) (ren_Val (shift)) tauVal) (fun x => eq_refl) (sigma fin_n))) ((ap) (ren_Val (shift)) (Eq fin_n)))
   | None  => eq_refl
   end.
 
-Fixpoint compSubstSubst_Val { kVal : nat } { lVal : nat } { m : nat } (sigmaVal : fin m -> Val (kVal)) (tauVal : fin (kVal) -> Val (lVal)) (thetaVal : fin m -> Val (lVal)) (EqVal : forall x, ((funcomp) (subst_Val tauVal) sigmaVal) x = thetaVal x) (s : Val m) : subst_Val tauVal (subst_Val sigmaVal s) = subst_Val thetaVal s :=
-  let fix compSubstSubst_Vals (vs : list (Val m)) :=
-    match vs  return subst_Vals tauVal (subst_Vals sigmaVal vs) = subst_Vals thetaVal vs with
-    | nil => eq_refl
-    | cons v vs' => congr_cons (compSubstSubst_Val sigmaVal tauVal thetaVal EqVal v)
-                              (compSubstSubst_Vals vs')
-    end in 
+Fixpoint compSubstSubst_Val { kVal : nat } { lVal : nat } { mVal : nat } (sigmaVal : (fin) (mVal) -> Val (kVal)) (tauVal : (fin) (kVal) -> Val (lVal)) (thetaVal : (fin) (mVal) -> Val (lVal)) (EqVal : forall x, ((funcomp) (subst_Val tauVal) sigmaVal) x = thetaVal x) (s : Val (mVal)) : subst_Val tauVal (subst_Val sigmaVal s) = subst_Val thetaVal s :=
     match s return subst_Val tauVal (subst_Val sigmaVal s) = subst_Val thetaVal s with
     | var_Val (_) s => EqVal s
     | Int (_) s0 => congr_Int ((fun x => (eq_refl) x) s0)
     | Prim (_) s0 => congr_Prim ((fun x => (eq_refl) x) s0)
-    | Tuple (_) s0 => congr_Tuple (compSubstSubst_Vals s0)
+    | Tuple (_) s0 => congr_Tuple ((list_comp (compSubstSubst_Val sigmaVal tauVal thetaVal EqVal)) s0)
     | Lam (_) s0 => congr_Lam ((compSubstSubst_Exp (up_Val_Val sigmaVal) (up_Val_Val tauVal) (up_Val_Val thetaVal) (up_subst_subst_Val_Val (_) (_) (_) EqVal)) s0)
     end
- with compSubstSubst_Exp { kVal : nat } { lVal : nat } { m : nat } (sigmaVal : fin m -> Val (kVal)) (tauVal : fin (kVal) -> Val (lVal)) (thetaVal : fin m -> Val (lVal)) (EqVal : forall x, ((funcomp) (subst_Val tauVal) sigmaVal) x = thetaVal x) (s : Exp m) : subst_Exp tauVal (subst_Exp sigmaVal s) = subst_Exp thetaVal s :=
+ with compSubstSubst_Exp { kVal : nat } { lVal : nat } { mVal : nat } (sigmaVal : (fin) (mVal) -> Val (kVal)) (tauVal : (fin) (kVal) -> Val (lVal)) (thetaVal : (fin) (mVal) -> Val (lVal)) (EqVal : forall x, ((funcomp) (subst_Val tauVal) sigmaVal) x = thetaVal x) (s : Exp (mVal)) : subst_Exp tauVal (subst_Exp sigmaVal s) = subst_Exp thetaVal s :=
     match s return subst_Exp tauVal (subst_Exp sigmaVal s) = subst_Exp thetaVal s with
     | Ret (_) s0 => congr_Ret ((compSubstSubst_Val sigmaVal tauVal thetaVal EqVal) s0)
     | App (_) s0 s1 => congr_App ((compSubstSubst_Val sigmaVal tauVal thetaVal EqVal) s0) ((compSubstSubst_Val sigmaVal tauVal thetaVal EqVal) s1)
@@ -368,26 +311,21 @@ Fixpoint compSubstSubst_Val { kVal : nat } { lVal : nat } { m : nat } (sigmaVal 
     | All (_) s0 => congr_All ((compSubstSubst_Exp sigmaVal tauVal thetaVal EqVal) s0)
     end.
 
-Definition rinstInst_up_Val_Val { m : nat } { n : nat } (xi : fin m -> fin n) (sigma : fin m -> Val n) (Eq : forall x, ((funcomp) (var_Val n) xi) x = sigma x) : forall x, ((funcomp) (var_Val (S n)) (upRen_Val_Val xi)) x = (up_Val_Val sigma) x :=
+Definition rinstInst_up_Val_Val { m : nat } { nVal : nat } (xi : (fin) (m) -> (fin) (nVal)) (sigma : (fin) (m) -> Val (nVal)) (Eq : forall x, ((funcomp) (var_Val (nVal)) xi) x = sigma x) : forall x, ((funcomp) (var_Val ((S) nVal)) (upRen_Val_Val xi)) x = (up_Val_Val sigma) x :=
   fun n => match n with
   | Some fin_n => (ap) (ren_Val (shift)) (Eq fin_n)
   | None  => eq_refl
   end.
 
-Fixpoint rinst_inst_Val { m : nat } { n : nat } (xiVal : fin m -> fin n) (sigmaVal : fin m -> Val n) (EqVal : forall x, ((funcomp) (var_Val n) xiVal) x = sigmaVal x) (s : Val m) : ren_Val xiVal s = subst_Val sigmaVal s :=
-  let fix rinst_inst_Vals (vs : list (Val m)) := 
-    match vs return ren_Vals xiVal vs = subst_Vals sigmaVal vs with
-    | nil => eq_refl
-    | cons v vs' => congr_cons (rinst_inst_Val xiVal sigmaVal EqVal v) (rinst_inst_Vals vs') 
-    end in
+Fixpoint rinst_inst_Val { mVal : nat } { nVal : nat } (xiVal : (fin) (mVal) -> (fin) (nVal)) (sigmaVal : (fin) (mVal) -> Val (nVal)) (EqVal : forall x, ((funcomp) (var_Val (nVal)) xiVal) x = sigmaVal x) (s : Val (mVal)) : ren_Val xiVal s = subst_Val sigmaVal s :=
     match s return ren_Val xiVal s = subst_Val sigmaVal s with
     | var_Val (_) s => EqVal s
     | Int (_) s0 => congr_Int ((fun x => (eq_refl) x) s0)
     | Prim (_) s0 => congr_Prim ((fun x => (eq_refl) x) s0)
-    | Tuple (_) s0 => congr_Tuple (rinst_inst_Vals s0)
+    | Tuple (_) s0 => congr_Tuple ((list_ext (rinst_inst_Val xiVal sigmaVal EqVal)) s0)
     | Lam (_) s0 => congr_Lam ((rinst_inst_Exp (upRen_Val_Val xiVal) (up_Val_Val sigmaVal) (rinstInst_up_Val_Val (_) (_) EqVal)) s0)
     end
- with rinst_inst_Exp { m : nat } { n : nat } (xiVal : fin m -> fin n) (sigmaVal : fin m -> Val n) (EqVal : forall x, ((funcomp) (var_Val n) xiVal) x = sigmaVal x) (s : Exp m) : ren_Exp xiVal s = subst_Exp sigmaVal s :=
+ with rinst_inst_Exp { mVal : nat } { nVal : nat } (xiVal : (fin) (mVal) -> (fin) (nVal)) (sigmaVal : (fin) (mVal) -> Val (nVal)) (EqVal : forall x, ((funcomp) (var_Val (nVal)) xiVal) x = sigmaVal x) (s : Exp (mVal)) : ren_Exp xiVal s = subst_Exp sigmaVal s :=
     match s return ren_Exp xiVal s = subst_Exp sigmaVal s with
     | Ret (_) s0 => congr_Ret ((rinst_inst_Val xiVal sigmaVal EqVal) s0)
     | App (_) s0 s1 => congr_App ((rinst_inst_Val xiVal sigmaVal EqVal) s0) ((rinst_inst_Val xiVal sigmaVal EqVal) s1)
@@ -400,123 +338,651 @@ Fixpoint rinst_inst_Val { m : nat } { n : nat } (xiVal : fin m -> fin n) (sigmaV
     | All (_) s0 => congr_All ((rinst_inst_Exp xiVal sigmaVal EqVal) s0)
     end.
 
-Lemma rinstInst_Val { m : nat } { n : nat } (xiVal : fin m -> fin n) : ren_Val xiVal = subst_Val ((funcomp) (var_Val n) xiVal) .
+Lemma rinstInst_Val { mVal : nat } { nVal : nat } (xiVal : (fin) (mVal) -> (fin) (nVal)) : ren_Val xiVal = subst_Val ((funcomp) (var_Val (nVal)) xiVal) .
 Proof. exact ((FunctionalExtensionality.functional_extensionality _ _ ) (fun x => rinst_inst_Val xiVal (_) (fun n => eq_refl) x)). Qed.
 
-Lemma rinstInst_Exp { m : nat } { n : nat } (xiVal : fin m -> fin n) : ren_Exp xiVal = subst_Exp ((funcomp) (var_Val n) xiVal) .
+Lemma rinstInst_Exp { mVal : nat } { nVal : nat } (xiVal : (fin) (mVal) -> (fin) (nVal)) : ren_Exp xiVal = subst_Exp ((funcomp) (var_Val (nVal)) xiVal) .
 Proof. exact ((FunctionalExtensionality.functional_extensionality _ _ ) (fun x => rinst_inst_Exp xiVal (_) (fun n => eq_refl) x)). Qed.
 
-Lemma instId_Val { m : nat } : subst_Val (var_Val m) = id .
-Proof. exact ((FunctionalExtensionality.functional_extensionality _ _ ) (fun x => idSubst_Val (var_Val m) (fun n => eq_refl) ((id) x))). Qed.
+Lemma instId_Val { mVal : nat } : subst_Val (var_Val (mVal)) = id .
+Proof. exact ((FunctionalExtensionality.functional_extensionality _ _ ) (fun x => idSubst_Val (var_Val (mVal)) (fun n => eq_refl) ((id) x))). Qed.
 
-Lemma instId_Exp { m : nat } : subst_Exp (var_Val m) = id .
-Proof. exact ((FunctionalExtensionality.functional_extensionality _ _ ) (fun x => idSubst_Exp (var_Val m) (fun n => eq_refl) ((id) x))). Qed.
+Lemma instId_Exp { mVal : nat } : subst_Exp (var_Val (mVal)) = id .
+Proof. exact ((FunctionalExtensionality.functional_extensionality _ _ ) (fun x => idSubst_Exp (var_Val (mVal)) (fun n => eq_refl) ((id) x))). Qed.
 
-Lemma rinstId_Val { m : nat } : @ren_Val m m (id) = id .
+Lemma rinstId_Val { mVal : nat } : @ren_Val (mVal) (mVal) (id) = id .
 Proof. exact ((eq_trans) (rinstInst_Val ((id) (_))) instId_Val). Qed.
 
-Lemma rinstId_Exp { m : nat } : @ren_Exp m m (id) = id .
+Lemma rinstId_Exp { mVal : nat } : @ren_Exp (mVal) (mVal) (id) = id .
 Proof. exact ((eq_trans) (rinstInst_Exp ((id) (_))) instId_Exp). Qed.
 
-Lemma varL_Val { m : nat } { n : nat } (sigmaVal : fin m -> Val n) : (funcomp) (subst_Val sigmaVal) (var_Val m) = sigmaVal .
+Lemma varL_Val { mVal : nat } { nVal : nat } (sigmaVal : (fin) (mVal) -> Val (nVal)) : (funcomp) (subst_Val sigmaVal) (var_Val (mVal)) = sigmaVal .
 Proof. exact ((FunctionalExtensionality.functional_extensionality _ _ ) (fun x => eq_refl)). Qed.
 
-Lemma varLRen_Val { m : nat } { n : nat } (xiVal : fin m -> fin n) : (funcomp) (ren_Val xiVal) (var_Val m) = (funcomp) (var_Val n) xiVal .
+Lemma varLRen_Val { mVal : nat } { nVal : nat } (xiVal : (fin) (mVal) -> (fin) (nVal)) : (funcomp) (ren_Val xiVal) (var_Val (mVal)) = (funcomp) (var_Val (nVal)) xiVal .
 Proof. exact ((FunctionalExtensionality.functional_extensionality _ _ ) (fun x => eq_refl)). Qed.
 
-Lemma compComp_Val { kVal : nat } { lVal : nat } { m : nat } (sigmaVal : fin m -> Val (kVal)) (tauVal : fin (kVal) -> Val (lVal)) (s : Val m) : subst_Val tauVal (subst_Val sigmaVal s) = subst_Val ((funcomp) (subst_Val tauVal) sigmaVal) s .
+Lemma compComp_Val { kVal : nat } { lVal : nat } { mVal : nat } (sigmaVal : (fin) (mVal) -> Val (kVal)) (tauVal : (fin) (kVal) -> Val (lVal)) (s : Val (mVal)) : subst_Val tauVal (subst_Val sigmaVal s) = subst_Val ((funcomp) (subst_Val tauVal) sigmaVal) s .
 Proof. exact (compSubstSubst_Val sigmaVal tauVal (_) (fun n => eq_refl) s). Qed.
 
-Lemma compComp_Exp { kVal : nat } { lVal : nat } { m : nat } (sigmaVal : fin m -> Val (kVal)) (tauVal : fin (kVal) -> Val (lVal)) (s : Exp m) : subst_Exp tauVal (subst_Exp sigmaVal s) = subst_Exp ((funcomp) (subst_Val tauVal) sigmaVal) s .
+Lemma compComp_Exp { kVal : nat } { lVal : nat } { mVal : nat } (sigmaVal : (fin) (mVal) -> Val (kVal)) (tauVal : (fin) (kVal) -> Val (lVal)) (s : Exp (mVal)) : subst_Exp tauVal (subst_Exp sigmaVal s) = subst_Exp ((funcomp) (subst_Val tauVal) sigmaVal) s .
 Proof. exact (compSubstSubst_Exp sigmaVal tauVal (_) (fun n => eq_refl) s). Qed.
 
-Lemma compComp'_Val { kVal : nat } { lVal : nat } { m : nat } (sigmaVal : fin m -> Val (kVal)) (tauVal : fin (kVal) -> Val (lVal)) : (funcomp) (subst_Val tauVal) (subst_Val sigmaVal) = subst_Val ((funcomp) (subst_Val tauVal) sigmaVal) .
+Lemma compComp'_Val { kVal : nat } { lVal : nat } { mVal : nat } (sigmaVal : (fin) (mVal) -> Val (kVal)) (tauVal : (fin) (kVal) -> Val (lVal)) : (funcomp) (subst_Val tauVal) (subst_Val sigmaVal) = subst_Val ((funcomp) (subst_Val tauVal) sigmaVal) .
 Proof. exact ((FunctionalExtensionality.functional_extensionality _ _ ) (fun n => compComp_Val sigmaVal tauVal n)). Qed.
 
-Lemma compComp'_Exp { kVal : nat } { lVal : nat } { m : nat } (sigmaVal : fin m -> Val (kVal)) (tauVal : fin (kVal) -> Val (lVal)) : (funcomp) (subst_Exp tauVal) (subst_Exp sigmaVal) = subst_Exp ((funcomp) (subst_Val tauVal) sigmaVal) .
+Lemma compComp'_Exp { kVal : nat } { lVal : nat } { mVal : nat } (sigmaVal : (fin) (mVal) -> Val (kVal)) (tauVal : (fin) (kVal) -> Val (lVal)) : (funcomp) (subst_Exp tauVal) (subst_Exp sigmaVal) = subst_Exp ((funcomp) (subst_Val tauVal) sigmaVal) .
 Proof. exact ((FunctionalExtensionality.functional_extensionality _ _ ) (fun n => compComp_Exp sigmaVal tauVal n)). Qed.
 
-Lemma compRen_Val { kVal : nat } { lVal : nat } { m : nat } (sigmaVal : fin m -> Val (kVal)) (zetaVal : fin (kVal) -> fin (lVal)) (s : Val m) : ren_Val zetaVal (subst_Val sigmaVal s) = subst_Val ((funcomp) (ren_Val zetaVal) sigmaVal) s .
+Lemma compRen_Val { kVal : nat } { lVal : nat } { mVal : nat } (sigmaVal : (fin) (mVal) -> Val (kVal)) (zetaVal : (fin) (kVal) -> (fin) (lVal)) (s : Val (mVal)) : ren_Val zetaVal (subst_Val sigmaVal s) = subst_Val ((funcomp) (ren_Val zetaVal) sigmaVal) s .
 Proof. exact (compSubstRen_Val sigmaVal zetaVal (_) (fun n => eq_refl) s). Qed.
 
-Lemma compRen_Exp { kVal : nat } { lVal : nat } { m : nat } (sigmaVal : fin m -> Val (kVal)) (zetaVal : fin (kVal) -> fin (lVal)) (s : Exp m) : ren_Exp zetaVal (subst_Exp sigmaVal s) = subst_Exp ((funcomp) (ren_Val zetaVal) sigmaVal) s .
+Lemma compRen_Exp { kVal : nat } { lVal : nat } { mVal : nat } (sigmaVal : (fin) (mVal) -> Val (kVal)) (zetaVal : (fin) (kVal) -> (fin) (lVal)) (s : Exp (mVal)) : ren_Exp zetaVal (subst_Exp sigmaVal s) = subst_Exp ((funcomp) (ren_Val zetaVal) sigmaVal) s .
 Proof. exact (compSubstRen_Exp sigmaVal zetaVal (_) (fun n => eq_refl) s). Qed.
 
-Lemma compRen'_Val { kVal : nat } { lVal : nat } { m : nat } (sigmaVal : fin m -> Val (kVal)) (zetaVal : fin (kVal) -> fin (lVal)) : (funcomp) (ren_Val zetaVal) (subst_Val sigmaVal) = subst_Val ((funcomp) (ren_Val zetaVal) sigmaVal) .
+Lemma compRen'_Val { kVal : nat } { lVal : nat } { mVal : nat } (sigmaVal : (fin) (mVal) -> Val (kVal)) (zetaVal : (fin) (kVal) -> (fin) (lVal)) : (funcomp) (ren_Val zetaVal) (subst_Val sigmaVal) = subst_Val ((funcomp) (ren_Val zetaVal) sigmaVal) .
 Proof. exact ((FunctionalExtensionality.functional_extensionality _ _ ) (fun n => compRen_Val sigmaVal zetaVal n)). Qed.
 
-Lemma compRen'_Exp { kVal : nat } { lVal : nat } { m : nat } (sigmaVal : fin m -> Val (kVal)) (zetaVal : fin (kVal) -> fin (lVal)) : (funcomp) (ren_Exp zetaVal) (subst_Exp sigmaVal) = subst_Exp ((funcomp) (ren_Val zetaVal) sigmaVal) .
+Lemma compRen'_Exp { kVal : nat } { lVal : nat } { mVal : nat } (sigmaVal : (fin) (mVal) -> Val (kVal)) (zetaVal : (fin) (kVal) -> (fin) (lVal)) : (funcomp) (ren_Exp zetaVal) (subst_Exp sigmaVal) = subst_Exp ((funcomp) (ren_Val zetaVal) sigmaVal) .
 Proof. exact ((FunctionalExtensionality.functional_extensionality _ _ ) (fun n => compRen_Exp sigmaVal zetaVal n)). Qed.
 
-Lemma renComp_Val { kVal : nat } { lVal : nat } { m : nat } (xiVal : fin m -> fin (kVal)) (tauVal : fin (kVal) -> Val (lVal)) (s : Val m) : subst_Val tauVal (ren_Val xiVal s) = subst_Val ((funcomp) tauVal xiVal) s .
+Lemma renComp_Val { kVal : nat } { lVal : nat } { mVal : nat } (xiVal : (fin) (mVal) -> (fin) (kVal)) (tauVal : (fin) (kVal) -> Val (lVal)) (s : Val (mVal)) : subst_Val tauVal (ren_Val xiVal s) = subst_Val ((funcomp) tauVal xiVal) s .
 Proof. exact (compRenSubst_Val xiVal tauVal (_) (fun n => eq_refl) s). Qed.
 
-Lemma renComp_Exp { kVal : nat } { lVal : nat } { m : nat } (xiVal : fin m -> fin (kVal)) (tauVal : fin (kVal) -> Val (lVal)) (s : Exp m) : subst_Exp tauVal (ren_Exp xiVal s) = subst_Exp ((funcomp) tauVal xiVal) s .
+Lemma renComp_Exp { kVal : nat } { lVal : nat } { mVal : nat } (xiVal : (fin) (mVal) -> (fin) (kVal)) (tauVal : (fin) (kVal) -> Val (lVal)) (s : Exp (mVal)) : subst_Exp tauVal (ren_Exp xiVal s) = subst_Exp ((funcomp) tauVal xiVal) s .
 Proof. exact (compRenSubst_Exp xiVal tauVal (_) (fun n => eq_refl) s). Qed.
 
-Lemma renComp'_Val { kVal : nat } { lVal : nat } { m : nat } (xiVal : fin m -> fin (kVal)) (tauVal : fin (kVal) -> Val (lVal)) : (funcomp) (subst_Val tauVal) (ren_Val xiVal) = subst_Val ((funcomp) tauVal xiVal) .
+Lemma renComp'_Val { kVal : nat } { lVal : nat } { mVal : nat } (xiVal : (fin) (mVal) -> (fin) (kVal)) (tauVal : (fin) (kVal) -> Val (lVal)) : (funcomp) (subst_Val tauVal) (ren_Val xiVal) = subst_Val ((funcomp) tauVal xiVal) .
 Proof. exact ((FunctionalExtensionality.functional_extensionality _ _ ) (fun n => renComp_Val xiVal tauVal n)). Qed.
 
-Lemma renComp'_Exp { kVal : nat } { lVal : nat } { m : nat } (xiVal : fin m -> fin (kVal)) (tauVal : fin (kVal) -> Val (lVal)) : (funcomp) (subst_Exp tauVal) (ren_Exp xiVal) = subst_Exp ((funcomp) tauVal xiVal) .
+Lemma renComp'_Exp { kVal : nat } { lVal : nat } { mVal : nat } (xiVal : (fin) (mVal) -> (fin) (kVal)) (tauVal : (fin) (kVal) -> Val (lVal)) : (funcomp) (subst_Exp tauVal) (ren_Exp xiVal) = subst_Exp ((funcomp) tauVal xiVal) .
 Proof. exact ((FunctionalExtensionality.functional_extensionality _ _ ) (fun n => renComp_Exp xiVal tauVal n)). Qed.
 
-Lemma renRen_Val { kVal : nat } { lVal : nat } { m : nat } (xiVal : fin m -> fin (kVal)) (zetaVal : fin (kVal) -> fin (lVal)) (s : Val m) : ren_Val zetaVal (ren_Val xiVal s) = ren_Val ((funcomp) zetaVal xiVal) s .
+Lemma renRen_Val { kVal : nat } { lVal : nat } { mVal : nat } (xiVal : (fin) (mVal) -> (fin) (kVal)) (zetaVal : (fin) (kVal) -> (fin) (lVal)) (s : Val (mVal)) : ren_Val zetaVal (ren_Val xiVal s) = ren_Val ((funcomp) zetaVal xiVal) s .
 Proof. exact (compRenRen_Val xiVal zetaVal (_) (fun n => eq_refl) s). Qed.
 
-Lemma renRen_Exp { kVal : nat } { lVal : nat } { m : nat } (xiVal : fin m -> fin (kVal)) (zetaVal : fin (kVal) -> fin (lVal)) (s : Exp m) : ren_Exp zetaVal (ren_Exp xiVal s) = ren_Exp ((funcomp) zetaVal xiVal) s .
+Lemma renRen_Exp { kVal : nat } { lVal : nat } { mVal : nat } (xiVal : (fin) (mVal) -> (fin) (kVal)) (zetaVal : (fin) (kVal) -> (fin) (lVal)) (s : Exp (mVal)) : ren_Exp zetaVal (ren_Exp xiVal s) = ren_Exp ((funcomp) zetaVal xiVal) s .
 Proof. exact (compRenRen_Exp xiVal zetaVal (_) (fun n => eq_refl) s). Qed.
 
-Lemma renRen'_Val { kVal : nat } { lVal : nat } { m : nat } (xiVal : fin m -> fin (kVal)) (zetaVal : fin (kVal) -> fin (lVal)) : (funcomp) (ren_Val zetaVal) (ren_Val xiVal) = ren_Val ((funcomp) zetaVal xiVal) .
+Lemma renRen'_Val { kVal : nat } { lVal : nat } { mVal : nat } (xiVal : (fin) (mVal) -> (fin) (kVal)) (zetaVal : (fin) (kVal) -> (fin) (lVal)) : (funcomp) (ren_Val zetaVal) (ren_Val xiVal) = ren_Val ((funcomp) zetaVal xiVal) .
 Proof. exact ((FunctionalExtensionality.functional_extensionality _ _ ) (fun n => renRen_Val xiVal zetaVal n)). Qed.
 
-Lemma renRen'_Exp { kVal : nat } { lVal : nat } { m : nat } (xiVal : fin m -> fin (kVal)) (zetaVal : fin (kVal) -> fin (lVal)) : (funcomp) (ren_Exp zetaVal) (ren_Exp xiVal) = ren_Exp ((funcomp) zetaVal xiVal) .
+Lemma renRen'_Exp { kVal : nat } { lVal : nat } { mVal : nat } (xiVal : (fin) (mVal) -> (fin) (kVal)) (zetaVal : (fin) (kVal) -> (fin) (lVal)) : (funcomp) (ren_Exp zetaVal) (ren_Exp xiVal) = ren_Exp ((funcomp) zetaVal xiVal) .
 Proof. exact ((FunctionalExtensionality.functional_extensionality _ _ ) (fun n => renRen_Exp xiVal zetaVal n)). Qed.
 
 End ValExp.
 
-Arguments var_Val {n}.
+Section SC.
+Inductive SC (nVal : nat) : Type :=
+  | SCchoicehole : SC (nVal)
+  | SCchoiceleft : SC  (nVal) -> Exp  (nVal) -> SC (nVal)
+  | SCchoiceright : Exp  (nVal) -> SC  (nVal) -> SC (nVal).
 
-Arguments Int {n}.
+Lemma congr_SCchoicehole { mVal : nat } : SCchoicehole (mVal) = SCchoicehole (mVal) .
+Proof. congruence. Qed.
 
-Arguments Prim {n}.
+Lemma congr_SCchoiceleft { mVal : nat } { s0 : SC  (mVal) } { s1 : Exp  (mVal) } { t0 : SC  (mVal) } { t1 : Exp  (mVal) } (H1 : s0 = t0) (H2 : s1 = t1) : SCchoiceleft (mVal) s0 s1 = SCchoiceleft (mVal) t0 t1 .
+Proof. congruence. Qed.
 
-Arguments Tuple {n}.
+Lemma congr_SCchoiceright { mVal : nat } { s0 : Exp  (mVal) } { s1 : SC  (mVal) } { t0 : Exp  (mVal) } { t1 : SC  (mVal) } (H1 : s0 = t0) (H2 : s1 = t1) : SCchoiceright (mVal) s0 s1 = SCchoiceright (mVal) t0 t1 .
+Proof. congruence. Qed.
 
-Arguments Lam {n}.
+Fixpoint subst_SC { mVal : nat } { nVal : nat } (sigmaVal : (fin) (mVal) -> Val (nVal)) (s : SC (mVal)) : SC (nVal) :=
+    match s return SC (nVal) with
+    | SCchoicehole (_)  => SCchoicehole (nVal)
+    | SCchoiceleft (_) s0 s1 => SCchoiceleft (nVal) ((subst_SC sigmaVal) s0) ((subst_Exp sigmaVal) s1)
+    | SCchoiceright (_) s0 s1 => SCchoiceright (nVal) ((subst_Exp sigmaVal) s0) ((subst_SC sigmaVal) s1)
+    end.
 
-Arguments Ret {n}.
+Fixpoint idSubst_SC { mVal : nat } (sigmaVal : (fin) (mVal) -> Val (mVal)) (EqVal : forall x, sigmaVal x = (var_Val (mVal)) x) (s : SC (mVal)) : subst_SC sigmaVal s = s :=
+    match s return subst_SC sigmaVal s = s with
+    | SCchoicehole (_)  => congr_SCchoicehole 
+    | SCchoiceleft (_) s0 s1 => congr_SCchoiceleft ((idSubst_SC sigmaVal EqVal) s0) ((idSubst_Exp sigmaVal EqVal) s1)
+    | SCchoiceright (_) s0 s1 => congr_SCchoiceright ((idSubst_Exp sigmaVal EqVal) s0) ((idSubst_SC sigmaVal EqVal) s1)
+    end.
 
-Arguments App {n}.
+Fixpoint ext_SC { mVal : nat } { nVal : nat } (sigmaVal : (fin) (mVal) -> Val (nVal)) (tauVal : (fin) (mVal) -> Val (nVal)) (EqVal : forall x, sigmaVal x = tauVal x) (s : SC (mVal)) : subst_SC sigmaVal s = subst_SC tauVal s :=
+    match s return subst_SC sigmaVal s = subst_SC tauVal s with
+    | SCchoicehole (_)  => congr_SCchoicehole 
+    | SCchoiceleft (_) s0 s1 => congr_SCchoiceleft ((ext_SC sigmaVal tauVal EqVal) s0) ((ext_Exp sigmaVal tauVal EqVal) s1)
+    | SCchoiceright (_) s0 s1 => congr_SCchoiceright ((ext_Exp sigmaVal tauVal EqVal) s0) ((ext_SC sigmaVal tauVal EqVal) s1)
+    end.
 
-Arguments Seq {n}.
+Fixpoint compSubstSubst_SC { kVal : nat } { lVal : nat } { mVal : nat } (sigmaVal : (fin) (mVal) -> Val (kVal)) (tauVal : (fin) (kVal) -> Val (lVal)) (thetaVal : (fin) (mVal) -> Val (lVal)) (EqVal : forall x, ((funcomp) (subst_Val tauVal) sigmaVal) x = thetaVal x) (s : SC (mVal)) : subst_SC tauVal (subst_SC sigmaVal s) = subst_SC thetaVal s :=
+    match s return subst_SC tauVal (subst_SC sigmaVal s) = subst_SC thetaVal s with
+    | SCchoicehole (_)  => congr_SCchoicehole 
+    | SCchoiceleft (_) s0 s1 => congr_SCchoiceleft ((compSubstSubst_SC sigmaVal tauVal thetaVal EqVal) s0) ((compSubstSubst_Exp sigmaVal tauVal thetaVal EqVal) s1)
+    | SCchoiceright (_) s0 s1 => congr_SCchoiceright ((compSubstSubst_Exp sigmaVal tauVal thetaVal EqVal) s0) ((compSubstSubst_SC sigmaVal tauVal thetaVal EqVal) s1)
+    end.
 
-Arguments Unify {n}.
+Lemma instId_SC { mVal : nat } : subst_SC (var_Val (mVal)) = id .
+Proof. exact ((FunctionalExtensionality.functional_extensionality _ _ ) (fun x => idSubst_SC (var_Val (mVal)) (fun n => eq_refl) ((id) x))). Qed.
 
-Arguments Exists {n}.
+Lemma compComp_SC { kVal : nat } { lVal : nat } { mVal : nat } (sigmaVal : (fin) (mVal) -> Val (kVal)) (tauVal : (fin) (kVal) -> Val (lVal)) (s : SC (mVal)) : subst_SC tauVal (subst_SC sigmaVal s) = subst_SC ((funcomp) (subst_Val tauVal) sigmaVal) s .
+Proof. exact (compSubstSubst_SC sigmaVal tauVal (_) (fun n => eq_refl) s). Qed.
 
-Arguments Or {n}.
+Lemma compComp'_SC { kVal : nat } { lVal : nat } { mVal : nat } (sigmaVal : (fin) (mVal) -> Val (kVal)) (tauVal : (fin) (kVal) -> Val (lVal)) : (funcomp) (subst_SC tauVal) (subst_SC sigmaVal) = subst_SC ((funcomp) (subst_Val tauVal) sigmaVal) .
+Proof. exact ((FunctionalExtensionality.functional_extensionality _ _ ) (fun n => compComp_SC sigmaVal tauVal n)). Qed.
 
-Arguments Fail {n}.
+End SC.
 
-Arguments One {n}.
+Section scopeContext.
+Inductive scopeContext (nVal : nat) : Type :=
+  | SXone : SC  (nVal) -> scopeContext (nVal)
+  | SXall : SC  (nVal) -> scopeContext (nVal).
 
-Arguments All {n}.
+Lemma congr_SXone { mVal : nat } { s0 : SC  (mVal) } { t0 : SC  (mVal) } (H1 : s0 = t0) : SXone (mVal) s0 = SXone (mVal) t0 .
+Proof. congruence. Qed.
 
-Global Instance Subst_Val { m : nat } { n : nat } : Subst1 (fin m -> Val n) (Val m) (Val n) := @subst_Val m n .
+Lemma congr_SXall { mVal : nat } { s0 : SC  (mVal) } { t0 : SC  (mVal) } (H1 : s0 = t0) : SXall (mVal) s0 = SXall (mVal) t0 .
+Proof. congruence. Qed.
 
-Global Instance Subst_Exp { m : nat } { n : nat } : Subst1 (fin m -> Val n) (Exp m) (Exp n) := @subst_Exp m n .
+Definition subst_scopeContext { mVal : nat } { nVal : nat } (sigmaVal : (fin) (mVal) -> Val (nVal)) (s : scopeContext (mVal)) : scopeContext (nVal) :=
+    match s return scopeContext (nVal) with
+    | SXone (_) s0 => SXone (nVal) ((subst_SC sigmaVal) s0)
+    | SXall (_) s0 => SXall (nVal) ((subst_SC sigmaVal) s0)
+    end.
 
-Global Instance Ren_Val { m : nat } { n : nat } : Ren1 (fin m -> fin n) (Val m) (Val n) := @ren_Val m n .
+Definition idSubst_scopeContext { mVal : nat } (sigmaVal : (fin) (mVal) -> Val (mVal)) (EqVal : forall x, sigmaVal x = (var_Val (mVal)) x) (s : scopeContext (mVal)) : subst_scopeContext sigmaVal s = s :=
+    match s return subst_scopeContext sigmaVal s = s with
+    | SXone (_) s0 => congr_SXone ((idSubst_SC sigmaVal EqVal) s0)
+    | SXall (_) s0 => congr_SXall ((idSubst_SC sigmaVal EqVal) s0)
+    end.
 
-Global Instance Ren_Exp { m : nat } { n : nat } : Ren1 (fin m -> fin n) (Exp m) (Exp n) := @ren_Exp m n .
+Definition ext_scopeContext { mVal : nat } { nVal : nat } (sigmaVal : (fin) (mVal) -> Val (nVal)) (tauVal : (fin) (mVal) -> Val (nVal)) (EqVal : forall x, sigmaVal x = tauVal x) (s : scopeContext (mVal)) : subst_scopeContext sigmaVal s = subst_scopeContext tauVal s :=
+    match s return subst_scopeContext sigmaVal s = subst_scopeContext tauVal s with
+    | SXone (_) s0 => congr_SXone ((ext_SC sigmaVal tauVal EqVal) s0)
+    | SXall (_) s0 => congr_SXall ((ext_SC sigmaVal tauVal EqVal) s0)
+    end.
 
-Global Instance VarInstance_Val { m : nat } : Var (fin m) (Val m) := @var_Val m .
+Definition compSubstSubst_scopeContext { kVal : nat } { lVal : nat } { mVal : nat } (sigmaVal : (fin) (mVal) -> Val (kVal)) (tauVal : (fin) (kVal) -> Val (lVal)) (thetaVal : (fin) (mVal) -> Val (lVal)) (EqVal : forall x, ((funcomp) (subst_Val tauVal) sigmaVal) x = thetaVal x) (s : scopeContext (mVal)) : subst_scopeContext tauVal (subst_scopeContext sigmaVal s) = subst_scopeContext thetaVal s :=
+    match s return subst_scopeContext tauVal (subst_scopeContext sigmaVal s) = subst_scopeContext thetaVal s with
+    | SXone (_) s0 => congr_SXone ((compSubstSubst_SC sigmaVal tauVal thetaVal EqVal) s0)
+    | SXall (_) s0 => congr_SXall ((compSubstSubst_SC sigmaVal tauVal thetaVal EqVal) s0)
+    end.
 
-Class Up_Val X Y := up_Val : X -> Y.
+Lemma instId_scopeContext { mVal : nat } : subst_scopeContext (var_Val (mVal)) = id .
+Proof. exact ((FunctionalExtensionality.functional_extensionality _ _ ) (fun x => idSubst_scopeContext (var_Val (mVal)) (fun n => eq_refl) ((id) x))). Qed.
 
-Global Instance Up_Val_Val { m : nat } { n : nat } : Up_Val (_) (_) := @up_Val_Val m n.
+Lemma compComp_scopeContext { kVal : nat } { lVal : nat } { mVal : nat } (sigmaVal : (fin) (mVal) -> Val (kVal)) (tauVal : (fin) (kVal) -> Val (lVal)) (s : scopeContext (mVal)) : subst_scopeContext tauVal (subst_scopeContext sigmaVal s) = subst_scopeContext ((funcomp) (subst_Val tauVal) sigmaVal) s .
+Proof. exact (compSubstSubst_scopeContext sigmaVal tauVal (_) (fun n => eq_refl) s). Qed.
 
-Module SubstNotations.
+Lemma compComp'_scopeContext { kVal : nat } { lVal : nat } { mVal : nat } (sigmaVal : (fin) (mVal) -> Val (kVal)) (tauVal : (fin) (kVal) -> Val (lVal)) : (funcomp) (subst_scopeContext tauVal) (subst_scopeContext sigmaVal) = subst_scopeContext ((funcomp) (subst_Val tauVal) sigmaVal) .
+Proof. exact ((FunctionalExtensionality.functional_extensionality _ _ ) (fun n => compComp_scopeContext sigmaVal tauVal n)). Qed.
+
+End scopeContext.
+
+Section ExpCompatContextValCompatContextValListCompatContext.
+Inductive ExpCompatContext (nVal : nat) : Type :=
+  | EHole : ExpCompatContext  (nVal) -> ExpCompatContext (nVal)
+  | ESeq1 : ExpCompatContext  (nVal) -> Exp  (nVal) -> ExpCompatContext (nVal)
+  | ESeq2 : Exp  (nVal) -> ExpCompatContext  (nVal) -> ExpCompatContext (nVal)
+  | EUnify1 : ValCompatContext  (nVal) -> Exp  (nVal) -> ExpCompatContext (nVal)
+  | EUnify2 : Val  (nVal) -> ExpCompatContext  (nVal) -> ExpCompatContext (nVal)
+  | EExists : ExpCompatContext  ((S) nVal) -> ExpCompatContext (nVal)
+  | EOr1 : ExpCompatContext  (nVal) -> Exp  (nVal) -> ExpCompatContext (nVal)
+  | EOr2 : Exp  (nVal) -> ExpCompatContext  (nVal) -> ExpCompatContext (nVal)
+  | EOne : ExpCompatContext  (nVal) -> ExpCompatContext (nVal)
+  | EAll : ExpCompatContext  (nVal) -> ExpCompatContext (nVal)
+  | EApp1 : ValCompatContext  (nVal) -> Val  (nVal) -> ExpCompatContext (nVal)
+  | EApp2 : Val  (nVal) -> ValCompatContext  (nVal) -> ExpCompatContext (nVal)
+  | ERet : ValCompatContext  (nVal) -> ExpCompatContext (nVal)
+ with ValCompatContext (nVal : nat) : Type :=
+  | VTuple : ValListCompatContext  (nVal) -> ValCompatContext (nVal)
+  | VLam : ExpCompatContext  ((S) nVal) -> ValCompatContext (nVal)
+ with ValListCompatContext (nVal : nat) : Type :=
+  | VEcons1 : ValCompatContext  (nVal) -> list (Val  (nVal)) -> ValListCompatContext (nVal)
+  | VEcons2 : Val  (nVal) -> ValListCompatContext  (nVal) -> ValListCompatContext (nVal).
+
+Lemma congr_EHole { mVal : nat } { s0 : ExpCompatContext  (mVal) } { t0 : ExpCompatContext  (mVal) } (H1 : s0 = t0) : EHole (mVal) s0 = EHole (mVal) t0 .
+Proof. congruence. Qed.
+
+Lemma congr_ESeq1 { mVal : nat } { s0 : ExpCompatContext  (mVal) } { s1 : Exp  (mVal) } { t0 : ExpCompatContext  (mVal) } { t1 : Exp  (mVal) } (H1 : s0 = t0) (H2 : s1 = t1) : ESeq1 (mVal) s0 s1 = ESeq1 (mVal) t0 t1 .
+Proof. congruence. Qed.
+
+Lemma congr_ESeq2 { mVal : nat } { s0 : Exp  (mVal) } { s1 : ExpCompatContext  (mVal) } { t0 : Exp  (mVal) } { t1 : ExpCompatContext  (mVal) } (H1 : s0 = t0) (H2 : s1 = t1) : ESeq2 (mVal) s0 s1 = ESeq2 (mVal) t0 t1 .
+Proof. congruence. Qed.
+
+Lemma congr_EUnify1 { mVal : nat } { s0 : ValCompatContext  (mVal) } { s1 : Exp  (mVal) } { t0 : ValCompatContext  (mVal) } { t1 : Exp  (mVal) } (H1 : s0 = t0) (H2 : s1 = t1) : EUnify1 (mVal) s0 s1 = EUnify1 (mVal) t0 t1 .
+Proof. congruence. Qed.
+
+Lemma congr_EUnify2 { mVal : nat } { s0 : Val  (mVal) } { s1 : ExpCompatContext  (mVal) } { t0 : Val  (mVal) } { t1 : ExpCompatContext  (mVal) } (H1 : s0 = t0) (H2 : s1 = t1) : EUnify2 (mVal) s0 s1 = EUnify2 (mVal) t0 t1 .
+Proof. congruence. Qed.
+
+Lemma congr_EExists { mVal : nat } { s0 : ExpCompatContext  ((S) mVal) } { t0 : ExpCompatContext  ((S) mVal) } (H1 : s0 = t0) : EExists (mVal) s0 = EExists (mVal) t0 .
+Proof. congruence. Qed.
+
+Lemma congr_EOr1 { mVal : nat } { s0 : ExpCompatContext  (mVal) } { s1 : Exp  (mVal) } { t0 : ExpCompatContext  (mVal) } { t1 : Exp  (mVal) } (H1 : s0 = t0) (H2 : s1 = t1) : EOr1 (mVal) s0 s1 = EOr1 (mVal) t0 t1 .
+Proof. congruence. Qed.
+
+Lemma congr_EOr2 { mVal : nat } { s0 : Exp  (mVal) } { s1 : ExpCompatContext  (mVal) } { t0 : Exp  (mVal) } { t1 : ExpCompatContext  (mVal) } (H1 : s0 = t0) (H2 : s1 = t1) : EOr2 (mVal) s0 s1 = EOr2 (mVal) t0 t1 .
+Proof. congruence. Qed.
+
+Lemma congr_EOne { mVal : nat } { s0 : ExpCompatContext  (mVal) } { t0 : ExpCompatContext  (mVal) } (H1 : s0 = t0) : EOne (mVal) s0 = EOne (mVal) t0 .
+Proof. congruence. Qed.
+
+Lemma congr_EAll { mVal : nat } { s0 : ExpCompatContext  (mVal) } { t0 : ExpCompatContext  (mVal) } (H1 : s0 = t0) : EAll (mVal) s0 = EAll (mVal) t0 .
+Proof. congruence. Qed.
+
+Lemma congr_EApp1 { mVal : nat } { s0 : ValCompatContext  (mVal) } { s1 : Val  (mVal) } { t0 : ValCompatContext  (mVal) } { t1 : Val  (mVal) } (H1 : s0 = t0) (H2 : s1 = t1) : EApp1 (mVal) s0 s1 = EApp1 (mVal) t0 t1 .
+Proof. congruence. Qed.
+
+Lemma congr_EApp2 { mVal : nat } { s0 : Val  (mVal) } { s1 : ValCompatContext  (mVal) } { t0 : Val  (mVal) } { t1 : ValCompatContext  (mVal) } (H1 : s0 = t0) (H2 : s1 = t1) : EApp2 (mVal) s0 s1 = EApp2 (mVal) t0 t1 .
+Proof. congruence. Qed.
+
+Lemma congr_ERet { mVal : nat } { s0 : ValCompatContext  (mVal) } { t0 : ValCompatContext  (mVal) } (H1 : s0 = t0) : ERet (mVal) s0 = ERet (mVal) t0 .
+Proof. congruence. Qed.
+
+Lemma congr_VTuple { mVal : nat } { s0 : ValListCompatContext  (mVal) } { t0 : ValListCompatContext  (mVal) } (H1 : s0 = t0) : VTuple (mVal) s0 = VTuple (mVal) t0 .
+Proof. congruence. Qed.
+
+Lemma congr_VLam { mVal : nat } { s0 : ExpCompatContext  ((S) mVal) } { t0 : ExpCompatContext  ((S) mVal) } (H1 : s0 = t0) : VLam (mVal) s0 = VLam (mVal) t0 .
+Proof. congruence. Qed.
+
+Lemma congr_VEcons1 { mVal : nat } { s0 : ValCompatContext  (mVal) } { s1 : list (Val  (mVal)) } { t0 : ValCompatContext  (mVal) } { t1 : list (Val  (mVal)) } (H1 : s0 = t0) (H2 : s1 = t1) : VEcons1 (mVal) s0 s1 = VEcons1 (mVal) t0 t1 .
+Proof. congruence. Qed.
+
+Lemma congr_VEcons2 { mVal : nat } { s0 : Val  (mVal) } { s1 : ValListCompatContext  (mVal) } { t0 : Val  (mVal) } { t1 : ValListCompatContext  (mVal) } (H1 : s0 = t0) (H2 : s1 = t1) : VEcons2 (mVal) s0 s1 = VEcons2 (mVal) t0 t1 .
+Proof. congruence. Qed.
+
+Fixpoint subst_ExpCompatContext { mVal : nat } { nVal : nat } (sigmaVal : (fin) (mVal) -> Val (nVal)) (s : ExpCompatContext (mVal)) : ExpCompatContext (nVal) :=
+    match s return ExpCompatContext (nVal) with
+    | EHole (_) s0 => EHole (nVal) ((subst_ExpCompatContext sigmaVal) s0)
+    | ESeq1 (_) s0 s1 => ESeq1 (nVal) ((subst_ExpCompatContext sigmaVal) s0) ((subst_Exp sigmaVal) s1)
+    | ESeq2 (_) s0 s1 => ESeq2 (nVal) ((subst_Exp sigmaVal) s0) ((subst_ExpCompatContext sigmaVal) s1)
+    | EUnify1 (_) s0 s1 => EUnify1 (nVal) ((subst_ValCompatContext sigmaVal) s0) ((subst_Exp sigmaVal) s1)
+    | EUnify2 (_) s0 s1 => EUnify2 (nVal) ((subst_Val sigmaVal) s0) ((subst_ExpCompatContext sigmaVal) s1)
+    | EExists (_) s0 => EExists (nVal) ((subst_ExpCompatContext (up_Val_Val sigmaVal)) s0)
+    | EOr1 (_) s0 s1 => EOr1 (nVal) ((subst_ExpCompatContext sigmaVal) s0) ((subst_Exp sigmaVal) s1)
+    | EOr2 (_) s0 s1 => EOr2 (nVal) ((subst_Exp sigmaVal) s0) ((subst_ExpCompatContext sigmaVal) s1)
+    | EOne (_) s0 => EOne (nVal) ((subst_ExpCompatContext sigmaVal) s0)
+    | EAll (_) s0 => EAll (nVal) ((subst_ExpCompatContext sigmaVal) s0)
+    | EApp1 (_) s0 s1 => EApp1 (nVal) ((subst_ValCompatContext sigmaVal) s0) ((subst_Val sigmaVal) s1)
+    | EApp2 (_) s0 s1 => EApp2 (nVal) ((subst_Val sigmaVal) s0) ((subst_ValCompatContext sigmaVal) s1)
+    | ERet (_) s0 => ERet (nVal) ((subst_ValCompatContext sigmaVal) s0)
+    end
+ with subst_ValCompatContext { mVal : nat } { nVal : nat } (sigmaVal : (fin) (mVal) -> Val (nVal)) (s : ValCompatContext (mVal)) : ValCompatContext (nVal) :=
+    match s return ValCompatContext (nVal) with
+    | VTuple (_) s0 => VTuple (nVal) ((subst_ValListCompatContext sigmaVal) s0)
+    | VLam (_) s0 => VLam (nVal) ((subst_ExpCompatContext (up_Val_Val sigmaVal)) s0)
+    end
+ with subst_ValListCompatContext { mVal : nat } { nVal : nat } (sigmaVal : (fin) (mVal) -> Val (nVal)) (s : ValListCompatContext (mVal)) : ValListCompatContext (nVal) :=
+    match s return ValListCompatContext (nVal) with
+    | VEcons1 (_) s0 s1 => VEcons1 (nVal) ((subst_ValCompatContext sigmaVal) s0) ((list_map (subst_Val sigmaVal)) s1)
+    | VEcons2 (_) s0 s1 => VEcons2 (nVal) ((subst_Val sigmaVal) s0) ((subst_ValListCompatContext sigmaVal) s1)
+    end.
+
+Fixpoint idSubst_ExpCompatContext { mVal : nat } (sigmaVal : (fin) (mVal) -> Val (mVal)) (EqVal : forall x, sigmaVal x = (var_Val (mVal)) x) (s : ExpCompatContext (mVal)) : subst_ExpCompatContext sigmaVal s = s :=
+    match s return subst_ExpCompatContext sigmaVal s = s with
+    | EHole (_) s0 => congr_EHole ((idSubst_ExpCompatContext sigmaVal EqVal) s0)
+    | ESeq1 (_) s0 s1 => congr_ESeq1 ((idSubst_ExpCompatContext sigmaVal EqVal) s0) ((idSubst_Exp sigmaVal EqVal) s1)
+    | ESeq2 (_) s0 s1 => congr_ESeq2 ((idSubst_Exp sigmaVal EqVal) s0) ((idSubst_ExpCompatContext sigmaVal EqVal) s1)
+    | EUnify1 (_) s0 s1 => congr_EUnify1 ((idSubst_ValCompatContext sigmaVal EqVal) s0) ((idSubst_Exp sigmaVal EqVal) s1)
+    | EUnify2 (_) s0 s1 => congr_EUnify2 ((idSubst_Val sigmaVal EqVal) s0) ((idSubst_ExpCompatContext sigmaVal EqVal) s1)
+    | EExists (_) s0 => congr_EExists ((idSubst_ExpCompatContext (up_Val_Val sigmaVal) (upId_Val_Val (_) EqVal)) s0)
+    | EOr1 (_) s0 s1 => congr_EOr1 ((idSubst_ExpCompatContext sigmaVal EqVal) s0) ((idSubst_Exp sigmaVal EqVal) s1)
+    | EOr2 (_) s0 s1 => congr_EOr2 ((idSubst_Exp sigmaVal EqVal) s0) ((idSubst_ExpCompatContext sigmaVal EqVal) s1)
+    | EOne (_) s0 => congr_EOne ((idSubst_ExpCompatContext sigmaVal EqVal) s0)
+    | EAll (_) s0 => congr_EAll ((idSubst_ExpCompatContext sigmaVal EqVal) s0)
+    | EApp1 (_) s0 s1 => congr_EApp1 ((idSubst_ValCompatContext sigmaVal EqVal) s0) ((idSubst_Val sigmaVal EqVal) s1)
+    | EApp2 (_) s0 s1 => congr_EApp2 ((idSubst_Val sigmaVal EqVal) s0) ((idSubst_ValCompatContext sigmaVal EqVal) s1)
+    | ERet (_) s0 => congr_ERet ((idSubst_ValCompatContext sigmaVal EqVal) s0)
+    end
+ with idSubst_ValCompatContext { mVal : nat } (sigmaVal : (fin) (mVal) -> Val (mVal)) (EqVal : forall x, sigmaVal x = (var_Val (mVal)) x) (s : ValCompatContext (mVal)) : subst_ValCompatContext sigmaVal s = s :=
+    match s return subst_ValCompatContext sigmaVal s = s with
+    | VTuple (_) s0 => congr_VTuple ((idSubst_ValListCompatContext sigmaVal EqVal) s0)
+    | VLam (_) s0 => congr_VLam ((idSubst_ExpCompatContext (up_Val_Val sigmaVal) (upId_Val_Val (_) EqVal)) s0)
+    end
+ with idSubst_ValListCompatContext { mVal : nat } (sigmaVal : (fin) (mVal) -> Val (mVal)) (EqVal : forall x, sigmaVal x = (var_Val (mVal)) x) (s : ValListCompatContext (mVal)) : subst_ValListCompatContext sigmaVal s = s :=
+    match s return subst_ValListCompatContext sigmaVal s = s with
+    | VEcons1 (_) s0 s1 => congr_VEcons1 ((idSubst_ValCompatContext sigmaVal EqVal) s0) ((list_id (idSubst_Val sigmaVal EqVal)) s1)
+    | VEcons2 (_) s0 s1 => congr_VEcons2 ((idSubst_Val sigmaVal EqVal) s0) ((idSubst_ValListCompatContext sigmaVal EqVal) s1)
+    end.
+
+Fixpoint ext_ExpCompatContext { mVal : nat } { nVal : nat } (sigmaVal : (fin) (mVal) -> Val (nVal)) (tauVal : (fin) (mVal) -> Val (nVal)) (EqVal : forall x, sigmaVal x = tauVal x) (s : ExpCompatContext (mVal)) : subst_ExpCompatContext sigmaVal s = subst_ExpCompatContext tauVal s :=
+    match s return subst_ExpCompatContext sigmaVal s = subst_ExpCompatContext tauVal s with
+    | EHole (_) s0 => congr_EHole ((ext_ExpCompatContext sigmaVal tauVal EqVal) s0)
+    | ESeq1 (_) s0 s1 => congr_ESeq1 ((ext_ExpCompatContext sigmaVal tauVal EqVal) s0) ((ext_Exp sigmaVal tauVal EqVal) s1)
+    | ESeq2 (_) s0 s1 => congr_ESeq2 ((ext_Exp sigmaVal tauVal EqVal) s0) ((ext_ExpCompatContext sigmaVal tauVal EqVal) s1)
+    | EUnify1 (_) s0 s1 => congr_EUnify1 ((ext_ValCompatContext sigmaVal tauVal EqVal) s0) ((ext_Exp sigmaVal tauVal EqVal) s1)
+    | EUnify2 (_) s0 s1 => congr_EUnify2 ((ext_Val sigmaVal tauVal EqVal) s0) ((ext_ExpCompatContext sigmaVal tauVal EqVal) s1)
+    | EExists (_) s0 => congr_EExists ((ext_ExpCompatContext (up_Val_Val sigmaVal) (up_Val_Val tauVal) (upExt_Val_Val (_) (_) EqVal)) s0)
+    | EOr1 (_) s0 s1 => congr_EOr1 ((ext_ExpCompatContext sigmaVal tauVal EqVal) s0) ((ext_Exp sigmaVal tauVal EqVal) s1)
+    | EOr2 (_) s0 s1 => congr_EOr2 ((ext_Exp sigmaVal tauVal EqVal) s0) ((ext_ExpCompatContext sigmaVal tauVal EqVal) s1)
+    | EOne (_) s0 => congr_EOne ((ext_ExpCompatContext sigmaVal tauVal EqVal) s0)
+    | EAll (_) s0 => congr_EAll ((ext_ExpCompatContext sigmaVal tauVal EqVal) s0)
+    | EApp1 (_) s0 s1 => congr_EApp1 ((ext_ValCompatContext sigmaVal tauVal EqVal) s0) ((ext_Val sigmaVal tauVal EqVal) s1)
+    | EApp2 (_) s0 s1 => congr_EApp2 ((ext_Val sigmaVal tauVal EqVal) s0) ((ext_ValCompatContext sigmaVal tauVal EqVal) s1)
+    | ERet (_) s0 => congr_ERet ((ext_ValCompatContext sigmaVal tauVal EqVal) s0)
+    end
+ with ext_ValCompatContext { mVal : nat } { nVal : nat } (sigmaVal : (fin) (mVal) -> Val (nVal)) (tauVal : (fin) (mVal) -> Val (nVal)) (EqVal : forall x, sigmaVal x = tauVal x) (s : ValCompatContext (mVal)) : subst_ValCompatContext sigmaVal s = subst_ValCompatContext tauVal s :=
+    match s return subst_ValCompatContext sigmaVal s = subst_ValCompatContext tauVal s with
+    | VTuple (_) s0 => congr_VTuple ((ext_ValListCompatContext sigmaVal tauVal EqVal) s0)
+    | VLam (_) s0 => congr_VLam ((ext_ExpCompatContext (up_Val_Val sigmaVal) (up_Val_Val tauVal) (upExt_Val_Val (_) (_) EqVal)) s0)
+    end
+ with ext_ValListCompatContext { mVal : nat } { nVal : nat } (sigmaVal : (fin) (mVal) -> Val (nVal)) (tauVal : (fin) (mVal) -> Val (nVal)) (EqVal : forall x, sigmaVal x = tauVal x) (s : ValListCompatContext (mVal)) : subst_ValListCompatContext sigmaVal s = subst_ValListCompatContext tauVal s :=
+    match s return subst_ValListCompatContext sigmaVal s = subst_ValListCompatContext tauVal s with
+    | VEcons1 (_) s0 s1 => congr_VEcons1 ((ext_ValCompatContext sigmaVal tauVal EqVal) s0) ((list_ext (ext_Val sigmaVal tauVal EqVal)) s1)
+    | VEcons2 (_) s0 s1 => congr_VEcons2 ((ext_Val sigmaVal tauVal EqVal) s0) ((ext_ValListCompatContext sigmaVal tauVal EqVal) s1)
+    end.
+
+Fixpoint compSubstSubst_ExpCompatContext { kVal : nat } { lVal : nat } { mVal : nat } (sigmaVal : (fin) (mVal) -> Val (kVal)) (tauVal : (fin) (kVal) -> Val (lVal)) (thetaVal : (fin) (mVal) -> Val (lVal)) (EqVal : forall x, ((funcomp) (subst_Val tauVal) sigmaVal) x = thetaVal x) (s : ExpCompatContext (mVal)) : subst_ExpCompatContext tauVal (subst_ExpCompatContext sigmaVal s) = subst_ExpCompatContext thetaVal s :=
+    match s return subst_ExpCompatContext tauVal (subst_ExpCompatContext sigmaVal s) = subst_ExpCompatContext thetaVal s with
+    | EHole (_) s0 => congr_EHole ((compSubstSubst_ExpCompatContext sigmaVal tauVal thetaVal EqVal) s0)
+    | ESeq1 (_) s0 s1 => congr_ESeq1 ((compSubstSubst_ExpCompatContext sigmaVal tauVal thetaVal EqVal) s0) ((compSubstSubst_Exp sigmaVal tauVal thetaVal EqVal) s1)
+    | ESeq2 (_) s0 s1 => congr_ESeq2 ((compSubstSubst_Exp sigmaVal tauVal thetaVal EqVal) s0) ((compSubstSubst_ExpCompatContext sigmaVal tauVal thetaVal EqVal) s1)
+    | EUnify1 (_) s0 s1 => congr_EUnify1 ((compSubstSubst_ValCompatContext sigmaVal tauVal thetaVal EqVal) s0) ((compSubstSubst_Exp sigmaVal tauVal thetaVal EqVal) s1)
+    | EUnify2 (_) s0 s1 => congr_EUnify2 ((compSubstSubst_Val sigmaVal tauVal thetaVal EqVal) s0) ((compSubstSubst_ExpCompatContext sigmaVal tauVal thetaVal EqVal) s1)
+    | EExists (_) s0 => congr_EExists ((compSubstSubst_ExpCompatContext (up_Val_Val sigmaVal) (up_Val_Val tauVal) (up_Val_Val thetaVal) (up_subst_subst_Val_Val (_) (_) (_) EqVal)) s0)
+    | EOr1 (_) s0 s1 => congr_EOr1 ((compSubstSubst_ExpCompatContext sigmaVal tauVal thetaVal EqVal) s0) ((compSubstSubst_Exp sigmaVal tauVal thetaVal EqVal) s1)
+    | EOr2 (_) s0 s1 => congr_EOr2 ((compSubstSubst_Exp sigmaVal tauVal thetaVal EqVal) s0) ((compSubstSubst_ExpCompatContext sigmaVal tauVal thetaVal EqVal) s1)
+    | EOne (_) s0 => congr_EOne ((compSubstSubst_ExpCompatContext sigmaVal tauVal thetaVal EqVal) s0)
+    | EAll (_) s0 => congr_EAll ((compSubstSubst_ExpCompatContext sigmaVal tauVal thetaVal EqVal) s0)
+    | EApp1 (_) s0 s1 => congr_EApp1 ((compSubstSubst_ValCompatContext sigmaVal tauVal thetaVal EqVal) s0) ((compSubstSubst_Val sigmaVal tauVal thetaVal EqVal) s1)
+    | EApp2 (_) s0 s1 => congr_EApp2 ((compSubstSubst_Val sigmaVal tauVal thetaVal EqVal) s0) ((compSubstSubst_ValCompatContext sigmaVal tauVal thetaVal EqVal) s1)
+    | ERet (_) s0 => congr_ERet ((compSubstSubst_ValCompatContext sigmaVal tauVal thetaVal EqVal) s0)
+    end
+ with compSubstSubst_ValCompatContext { kVal : nat } { lVal : nat } { mVal : nat } (sigmaVal : (fin) (mVal) -> Val (kVal)) (tauVal : (fin) (kVal) -> Val (lVal)) (thetaVal : (fin) (mVal) -> Val (lVal)) (EqVal : forall x, ((funcomp) (subst_Val tauVal) sigmaVal) x = thetaVal x) (s : ValCompatContext (mVal)) : subst_ValCompatContext tauVal (subst_ValCompatContext sigmaVal s) = subst_ValCompatContext thetaVal s :=
+    match s return subst_ValCompatContext tauVal (subst_ValCompatContext sigmaVal s) = subst_ValCompatContext thetaVal s with
+    | VTuple (_) s0 => congr_VTuple ((compSubstSubst_ValListCompatContext sigmaVal tauVal thetaVal EqVal) s0)
+    | VLam (_) s0 => congr_VLam ((compSubstSubst_ExpCompatContext (up_Val_Val sigmaVal) (up_Val_Val tauVal) (up_Val_Val thetaVal) (up_subst_subst_Val_Val (_) (_) (_) EqVal)) s0)
+    end
+ with compSubstSubst_ValListCompatContext { kVal : nat } { lVal : nat } { mVal : nat } (sigmaVal : (fin) (mVal) -> Val (kVal)) (tauVal : (fin) (kVal) -> Val (lVal)) (thetaVal : (fin) (mVal) -> Val (lVal)) (EqVal : forall x, ((funcomp) (subst_Val tauVal) sigmaVal) x = thetaVal x) (s : ValListCompatContext (mVal)) : subst_ValListCompatContext tauVal (subst_ValListCompatContext sigmaVal s) = subst_ValListCompatContext thetaVal s :=
+    match s return subst_ValListCompatContext tauVal (subst_ValListCompatContext sigmaVal s) = subst_ValListCompatContext thetaVal s with
+    | VEcons1 (_) s0 s1 => congr_VEcons1 ((compSubstSubst_ValCompatContext sigmaVal tauVal thetaVal EqVal) s0) ((list_comp (compSubstSubst_Val sigmaVal tauVal thetaVal EqVal)) s1)
+    | VEcons2 (_) s0 s1 => congr_VEcons2 ((compSubstSubst_Val sigmaVal tauVal thetaVal EqVal) s0) ((compSubstSubst_ValListCompatContext sigmaVal tauVal thetaVal EqVal) s1)
+    end.
+
+Lemma instId_ExpCompatContext { mVal : nat } : subst_ExpCompatContext (var_Val (mVal)) = id .
+Proof. exact ((FunctionalExtensionality.functional_extensionality _ _ ) (fun x => idSubst_ExpCompatContext (var_Val (mVal)) (fun n => eq_refl) ((id) x))). Qed.
+
+Lemma instId_ValCompatContext { mVal : nat } : subst_ValCompatContext (var_Val (mVal)) = id .
+Proof. exact ((FunctionalExtensionality.functional_extensionality _ _ ) (fun x => idSubst_ValCompatContext (var_Val (mVal)) (fun n => eq_refl) ((id) x))). Qed.
+
+Lemma instId_ValListCompatContext { mVal : nat } : subst_ValListCompatContext (var_Val (mVal)) = id .
+Proof. exact ((FunctionalExtensionality.functional_extensionality _ _ ) (fun x => idSubst_ValListCompatContext (var_Val (mVal)) (fun n => eq_refl) ((id) x))). Qed.
+
+Lemma compComp_ExpCompatContext { kVal : nat } { lVal : nat } { mVal : nat } (sigmaVal : (fin) (mVal) -> Val (kVal)) (tauVal : (fin) (kVal) -> Val (lVal)) (s : ExpCompatContext (mVal)) : subst_ExpCompatContext tauVal (subst_ExpCompatContext sigmaVal s) = subst_ExpCompatContext ((funcomp) (subst_Val tauVal) sigmaVal) s .
+Proof. exact (compSubstSubst_ExpCompatContext sigmaVal tauVal (_) (fun n => eq_refl) s). Qed.
+
+Lemma compComp_ValCompatContext { kVal : nat } { lVal : nat } { mVal : nat } (sigmaVal : (fin) (mVal) -> Val (kVal)) (tauVal : (fin) (kVal) -> Val (lVal)) (s : ValCompatContext (mVal)) : subst_ValCompatContext tauVal (subst_ValCompatContext sigmaVal s) = subst_ValCompatContext ((funcomp) (subst_Val tauVal) sigmaVal) s .
+Proof. exact (compSubstSubst_ValCompatContext sigmaVal tauVal (_) (fun n => eq_refl) s). Qed.
+
+Lemma compComp_ValListCompatContext { kVal : nat } { lVal : nat } { mVal : nat } (sigmaVal : (fin) (mVal) -> Val (kVal)) (tauVal : (fin) (kVal) -> Val (lVal)) (s : ValListCompatContext (mVal)) : subst_ValListCompatContext tauVal (subst_ValListCompatContext sigmaVal s) = subst_ValListCompatContext ((funcomp) (subst_Val tauVal) sigmaVal) s .
+Proof. exact (compSubstSubst_ValListCompatContext sigmaVal tauVal (_) (fun n => eq_refl) s). Qed.
+
+Lemma compComp'_ExpCompatContext { kVal : nat } { lVal : nat } { mVal : nat } (sigmaVal : (fin) (mVal) -> Val (kVal)) (tauVal : (fin) (kVal) -> Val (lVal)) : (funcomp) (subst_ExpCompatContext tauVal) (subst_ExpCompatContext sigmaVal) = subst_ExpCompatContext ((funcomp) (subst_Val tauVal) sigmaVal) .
+Proof. exact ((FunctionalExtensionality.functional_extensionality _ _ ) (fun n => compComp_ExpCompatContext sigmaVal tauVal n)). Qed.
+
+Lemma compComp'_ValCompatContext { kVal : nat } { lVal : nat } { mVal : nat } (sigmaVal : (fin) (mVal) -> Val (kVal)) (tauVal : (fin) (kVal) -> Val (lVal)) : (funcomp) (subst_ValCompatContext tauVal) (subst_ValCompatContext sigmaVal) = subst_ValCompatContext ((funcomp) (subst_Val tauVal) sigmaVal) .
+Proof. exact ((FunctionalExtensionality.functional_extensionality _ _ ) (fun n => compComp_ValCompatContext sigmaVal tauVal n)). Qed.
+
+Lemma compComp'_ValListCompatContext { kVal : nat } { lVal : nat } { mVal : nat } (sigmaVal : (fin) (mVal) -> Val (kVal)) (tauVal : (fin) (kVal) -> Val (lVal)) : (funcomp) (subst_ValListCompatContext tauVal) (subst_ValListCompatContext sigmaVal) = subst_ValListCompatContext ((funcomp) (subst_Val tauVal) sigmaVal) .
+Proof. exact ((FunctionalExtensionality.functional_extensionality _ _ ) (fun n => compComp_ValListCompatContext sigmaVal tauVal n)). Qed.
+
+End ExpCompatContextValCompatContextValListCompatContext.
+
+Section choiceContext.
+Inductive choiceContext (nVal : nat) : Type :=
+  | CXhole : choiceContext (nVal)
+  | CXchoiceright : Val  (nVal) -> choiceContext  (nVal) -> Exp  (nVal) -> choiceContext (nVal)
+  | CXseqleft : choiceContext  (nVal) -> Exp  (nVal) -> choiceContext (nVal)
+  | CXseqright : Exp  (nVal) -> choiceContext  (nVal) -> choiceContext (nVal)
+  | CXexists : choiceContext  ((S) nVal) -> choiceContext (nVal).
+
+Lemma congr_CXhole { mVal : nat } : CXhole (mVal) = CXhole (mVal) .
+Proof. congruence. Qed.
+
+Lemma congr_CXchoiceright { mVal : nat } { s0 : Val  (mVal) } { s1 : choiceContext  (mVal) } { s2 : Exp  (mVal) } { t0 : Val  (mVal) } { t1 : choiceContext  (mVal) } { t2 : Exp  (mVal) } (H1 : s0 = t0) (H2 : s1 = t1) (H3 : s2 = t2) : CXchoiceright (mVal) s0 s1 s2 = CXchoiceright (mVal) t0 t1 t2 .
+Proof. congruence. Qed.
+
+Lemma congr_CXseqleft { mVal : nat } { s0 : choiceContext  (mVal) } { s1 : Exp  (mVal) } { t0 : choiceContext  (mVal) } { t1 : Exp  (mVal) } (H1 : s0 = t0) (H2 : s1 = t1) : CXseqleft (mVal) s0 s1 = CXseqleft (mVal) t0 t1 .
+Proof. congruence. Qed.
+
+Lemma congr_CXseqright { mVal : nat } { s0 : Exp  (mVal) } { s1 : choiceContext  (mVal) } { t0 : Exp  (mVal) } { t1 : choiceContext  (mVal) } (H1 : s0 = t0) (H2 : s1 = t1) : CXseqright (mVal) s0 s1 = CXseqright (mVal) t0 t1 .
+Proof. congruence. Qed.
+
+Lemma congr_CXexists { mVal : nat } { s0 : choiceContext  ((S) mVal) } { t0 : choiceContext  ((S) mVal) } (H1 : s0 = t0) : CXexists (mVal) s0 = CXexists (mVal) t0 .
+Proof. congruence. Qed.
+
+Fixpoint subst_choiceContext { mVal : nat } { nVal : nat } (sigmaVal : (fin) (mVal) -> Val (nVal)) (s : choiceContext (mVal)) : choiceContext (nVal) :=
+    match s return choiceContext (nVal) with
+    | CXhole (_)  => CXhole (nVal)
+    | CXchoiceright (_) s0 s1 s2 => CXchoiceright (nVal) ((subst_Val sigmaVal) s0) ((subst_choiceContext sigmaVal) s1) ((subst_Exp sigmaVal) s2)
+    | CXseqleft (_) s0 s1 => CXseqleft (nVal) ((subst_choiceContext sigmaVal) s0) ((subst_Exp sigmaVal) s1)
+    | CXseqright (_) s0 s1 => CXseqright (nVal) ((subst_Exp sigmaVal) s0) ((subst_choiceContext sigmaVal) s1)
+    | CXexists (_) s0 => CXexists (nVal) ((subst_choiceContext (up_Val_Val sigmaVal)) s0)
+    end.
+
+Fixpoint idSubst_choiceContext { mVal : nat } (sigmaVal : (fin) (mVal) -> Val (mVal)) (EqVal : forall x, sigmaVal x = (var_Val (mVal)) x) (s : choiceContext (mVal)) : subst_choiceContext sigmaVal s = s :=
+    match s return subst_choiceContext sigmaVal s = s with
+    | CXhole (_)  => congr_CXhole 
+    | CXchoiceright (_) s0 s1 s2 => congr_CXchoiceright ((idSubst_Val sigmaVal EqVal) s0) ((idSubst_choiceContext sigmaVal EqVal) s1) ((idSubst_Exp sigmaVal EqVal) s2)
+    | CXseqleft (_) s0 s1 => congr_CXseqleft ((idSubst_choiceContext sigmaVal EqVal) s0) ((idSubst_Exp sigmaVal EqVal) s1)
+    | CXseqright (_) s0 s1 => congr_CXseqright ((idSubst_Exp sigmaVal EqVal) s0) ((idSubst_choiceContext sigmaVal EqVal) s1)
+    | CXexists (_) s0 => congr_CXexists ((idSubst_choiceContext (up_Val_Val sigmaVal) (upId_Val_Val (_) EqVal)) s0)
+    end.
+
+Fixpoint ext_choiceContext { mVal : nat } { nVal : nat } (sigmaVal : (fin) (mVal) -> Val (nVal)) (tauVal : (fin) (mVal) -> Val (nVal)) (EqVal : forall x, sigmaVal x = tauVal x) (s : choiceContext (mVal)) : subst_choiceContext sigmaVal s = subst_choiceContext tauVal s :=
+    match s return subst_choiceContext sigmaVal s = subst_choiceContext tauVal s with
+    | CXhole (_)  => congr_CXhole 
+    | CXchoiceright (_) s0 s1 s2 => congr_CXchoiceright ((ext_Val sigmaVal tauVal EqVal) s0) ((ext_choiceContext sigmaVal tauVal EqVal) s1) ((ext_Exp sigmaVal tauVal EqVal) s2)
+    | CXseqleft (_) s0 s1 => congr_CXseqleft ((ext_choiceContext sigmaVal tauVal EqVal) s0) ((ext_Exp sigmaVal tauVal EqVal) s1)
+    | CXseqright (_) s0 s1 => congr_CXseqright ((ext_Exp sigmaVal tauVal EqVal) s0) ((ext_choiceContext sigmaVal tauVal EqVal) s1)
+    | CXexists (_) s0 => congr_CXexists ((ext_choiceContext (up_Val_Val sigmaVal) (up_Val_Val tauVal) (upExt_Val_Val (_) (_) EqVal)) s0)
+    end.
+
+Fixpoint compSubstSubst_choiceContext { kVal : nat } { lVal : nat } { mVal : nat } (sigmaVal : (fin) (mVal) -> Val (kVal)) (tauVal : (fin) (kVal) -> Val (lVal)) (thetaVal : (fin) (mVal) -> Val (lVal)) (EqVal : forall x, ((funcomp) (subst_Val tauVal) sigmaVal) x = thetaVal x) (s : choiceContext (mVal)) : subst_choiceContext tauVal (subst_choiceContext sigmaVal s) = subst_choiceContext thetaVal s :=
+    match s return subst_choiceContext tauVal (subst_choiceContext sigmaVal s) = subst_choiceContext thetaVal s with
+    | CXhole (_)  => congr_CXhole 
+    | CXchoiceright (_) s0 s1 s2 => congr_CXchoiceright ((compSubstSubst_Val sigmaVal tauVal thetaVal EqVal) s0) ((compSubstSubst_choiceContext sigmaVal tauVal thetaVal EqVal) s1) ((compSubstSubst_Exp sigmaVal tauVal thetaVal EqVal) s2)
+    | CXseqleft (_) s0 s1 => congr_CXseqleft ((compSubstSubst_choiceContext sigmaVal tauVal thetaVal EqVal) s0) ((compSubstSubst_Exp sigmaVal tauVal thetaVal EqVal) s1)
+    | CXseqright (_) s0 s1 => congr_CXseqright ((compSubstSubst_Exp sigmaVal tauVal thetaVal EqVal) s0) ((compSubstSubst_choiceContext sigmaVal tauVal thetaVal EqVal) s1)
+    | CXexists (_) s0 => congr_CXexists ((compSubstSubst_choiceContext (up_Val_Val sigmaVal) (up_Val_Val tauVal) (up_Val_Val thetaVal) (up_subst_subst_Val_Val (_) (_) (_) EqVal)) s0)
+    end.
+
+Lemma instId_choiceContext { mVal : nat } : subst_choiceContext (var_Val (mVal)) = id .
+Proof. exact ((FunctionalExtensionality.functional_extensionality _ _ ) (fun x => idSubst_choiceContext (var_Val (mVal)) (fun n => eq_refl) ((id) x))). Qed.
+
+Lemma compComp_choiceContext { kVal : nat } { lVal : nat } { mVal : nat } (sigmaVal : (fin) (mVal) -> Val (kVal)) (tauVal : (fin) (kVal) -> Val (lVal)) (s : choiceContext (mVal)) : subst_choiceContext tauVal (subst_choiceContext sigmaVal s) = subst_choiceContext ((funcomp) (subst_Val tauVal) sigmaVal) s .
+Proof. exact (compSubstSubst_choiceContext sigmaVal tauVal (_) (fun n => eq_refl) s). Qed.
+
+Lemma compComp'_choiceContext { kVal : nat } { lVal : nat } { mVal : nat } (sigmaVal : (fin) (mVal) -> Val (kVal)) (tauVal : (fin) (kVal) -> Val (lVal)) : (funcomp) (subst_choiceContext tauVal) (subst_choiceContext sigmaVal) = subst_choiceContext ((funcomp) (subst_Val tauVal) sigmaVal) .
+Proof. exact ((FunctionalExtensionality.functional_extensionality _ _ ) (fun n => compComp_choiceContext sigmaVal tauVal n)). Qed.
+
+End choiceContext.
+
+Section exContext.
+Inductive exContext (nVal : nat) : Type :=
+  | Xhole : exContext (nVal)
+  | Xeqright : Val  (nVal) -> exContext  (nVal) -> Exp  (nVal) -> exContext (nVal)
+  | Xseqleft : exContext  (nVal) -> Exp  (nVal) -> exContext (nVal)
+  | Xseqright : Exp  (nVal) -> exContext  (nVal) -> exContext (nVal).
+
+Lemma congr_Xhole { mVal : nat } : Xhole (mVal) = Xhole (mVal) .
+Proof. congruence. Qed.
+
+Lemma congr_Xeqright { mVal : nat } { s0 : Val  (mVal) } { s1 : exContext  (mVal) } { s2 : Exp  (mVal) } { t0 : Val  (mVal) } { t1 : exContext  (mVal) } { t2 : Exp  (mVal) } (H1 : s0 = t0) (H2 : s1 = t1) (H3 : s2 = t2) : Xeqright (mVal) s0 s1 s2 = Xeqright (mVal) t0 t1 t2 .
+Proof. congruence. Qed.
+
+Lemma congr_Xseqleft { mVal : nat } { s0 : exContext  (mVal) } { s1 : Exp  (mVal) } { t0 : exContext  (mVal) } { t1 : Exp  (mVal) } (H1 : s0 = t0) (H2 : s1 = t1) : Xseqleft (mVal) s0 s1 = Xseqleft (mVal) t0 t1 .
+Proof. congruence. Qed.
+
+Lemma congr_Xseqright { mVal : nat } { s0 : Exp  (mVal) } { s1 : exContext  (mVal) } { t0 : Exp  (mVal) } { t1 : exContext  (mVal) } (H1 : s0 = t0) (H2 : s1 = t1) : Xseqright (mVal) s0 s1 = Xseqright (mVal) t0 t1 .
+Proof. congruence. Qed.
+
+Fixpoint subst_exContext { mVal : nat } { nVal : nat } (sigmaVal : (fin) (mVal) -> Val (nVal)) (s : exContext (mVal)) : exContext (nVal) :=
+    match s return exContext (nVal) with
+    | Xhole (_)  => Xhole (nVal)
+    | Xeqright (_) s0 s1 s2 => Xeqright (nVal) ((subst_Val sigmaVal) s0) ((subst_exContext sigmaVal) s1) ((subst_Exp sigmaVal) s2)
+    | Xseqleft (_) s0 s1 => Xseqleft (nVal) ((subst_exContext sigmaVal) s0) ((subst_Exp sigmaVal) s1)
+    | Xseqright (_) s0 s1 => Xseqright (nVal) ((subst_Exp sigmaVal) s0) ((subst_exContext sigmaVal) s1)
+    end.
+
+Fixpoint idSubst_exContext { mVal : nat } (sigmaVal : (fin) (mVal) -> Val (mVal)) (EqVal : forall x, sigmaVal x = (var_Val (mVal)) x) (s : exContext (mVal)) : subst_exContext sigmaVal s = s :=
+    match s return subst_exContext sigmaVal s = s with
+    | Xhole (_)  => congr_Xhole 
+    | Xeqright (_) s0 s1 s2 => congr_Xeqright ((idSubst_Val sigmaVal EqVal) s0) ((idSubst_exContext sigmaVal EqVal) s1) ((idSubst_Exp sigmaVal EqVal) s2)
+    | Xseqleft (_) s0 s1 => congr_Xseqleft ((idSubst_exContext sigmaVal EqVal) s0) ((idSubst_Exp sigmaVal EqVal) s1)
+    | Xseqright (_) s0 s1 => congr_Xseqright ((idSubst_Exp sigmaVal EqVal) s0) ((idSubst_exContext sigmaVal EqVal) s1)
+    end.
+
+Fixpoint ext_exContext { mVal : nat } { nVal : nat } (sigmaVal : (fin) (mVal) -> Val (nVal)) (tauVal : (fin) (mVal) -> Val (nVal)) (EqVal : forall x, sigmaVal x = tauVal x) (s : exContext (mVal)) : subst_exContext sigmaVal s = subst_exContext tauVal s :=
+    match s return subst_exContext sigmaVal s = subst_exContext tauVal s with
+    | Xhole (_)  => congr_Xhole 
+    | Xeqright (_) s0 s1 s2 => congr_Xeqright ((ext_Val sigmaVal tauVal EqVal) s0) ((ext_exContext sigmaVal tauVal EqVal) s1) ((ext_Exp sigmaVal tauVal EqVal) s2)
+    | Xseqleft (_) s0 s1 => congr_Xseqleft ((ext_exContext sigmaVal tauVal EqVal) s0) ((ext_Exp sigmaVal tauVal EqVal) s1)
+    | Xseqright (_) s0 s1 => congr_Xseqright ((ext_Exp sigmaVal tauVal EqVal) s0) ((ext_exContext sigmaVal tauVal EqVal) s1)
+    end.
+
+Fixpoint compSubstSubst_exContext { kVal : nat } { lVal : nat } { mVal : nat } (sigmaVal : (fin) (mVal) -> Val (kVal)) (tauVal : (fin) (kVal) -> Val (lVal)) (thetaVal : (fin) (mVal) -> Val (lVal)) (EqVal : forall x, ((funcomp) (subst_Val tauVal) sigmaVal) x = thetaVal x) (s : exContext (mVal)) : subst_exContext tauVal (subst_exContext sigmaVal s) = subst_exContext thetaVal s :=
+    match s return subst_exContext tauVal (subst_exContext sigmaVal s) = subst_exContext thetaVal s with
+    | Xhole (_)  => congr_Xhole 
+    | Xeqright (_) s0 s1 s2 => congr_Xeqright ((compSubstSubst_Val sigmaVal tauVal thetaVal EqVal) s0) ((compSubstSubst_exContext sigmaVal tauVal thetaVal EqVal) s1) ((compSubstSubst_Exp sigmaVal tauVal thetaVal EqVal) s2)
+    | Xseqleft (_) s0 s1 => congr_Xseqleft ((compSubstSubst_exContext sigmaVal tauVal thetaVal EqVal) s0) ((compSubstSubst_Exp sigmaVal tauVal thetaVal EqVal) s1)
+    | Xseqright (_) s0 s1 => congr_Xseqright ((compSubstSubst_Exp sigmaVal tauVal thetaVal EqVal) s0) ((compSubstSubst_exContext sigmaVal tauVal thetaVal EqVal) s1)
+    end.
+
+Lemma instId_exContext { mVal : nat } : subst_exContext (var_Val (mVal)) = id .
+Proof. exact ((FunctionalExtensionality.functional_extensionality _ _ ) (fun x => idSubst_exContext (var_Val (mVal)) (fun n => eq_refl) ((id) x))). Qed.
+
+Lemma compComp_exContext { kVal : nat } { lVal : nat } { mVal : nat } (sigmaVal : (fin) (mVal) -> Val (kVal)) (tauVal : (fin) (kVal) -> Val (lVal)) (s : exContext (mVal)) : subst_exContext tauVal (subst_exContext sigmaVal s) = subst_exContext ((funcomp) (subst_Val tauVal) sigmaVal) s .
+Proof. exact (compSubstSubst_exContext sigmaVal tauVal (_) (fun n => eq_refl) s). Qed.
+
+Lemma compComp'_exContext { kVal : nat } { lVal : nat } { mVal : nat } (sigmaVal : (fin) (mVal) -> Val (kVal)) (tauVal : (fin) (kVal) -> Val (lVal)) : (funcomp) (subst_exContext tauVal) (subst_exContext sigmaVal) = subst_exContext ((funcomp) (subst_Val tauVal) sigmaVal) .
+Proof. exact ((FunctionalExtensionality.functional_extensionality _ _ ) (fun n => compComp_exContext sigmaVal tauVal n)). Qed.
+
+End exContext.
+
+Arguments var_Val {nVal}.
+
+Arguments Int {nVal}.
+
+Arguments Prim {nVal}.
+
+Arguments Tuple {nVal}.
+
+Arguments Lam {nVal}.
+
+Arguments Ret {nVal}.
+
+Arguments App {nVal}.
+
+Arguments Seq {nVal}.
+
+Arguments Unify {nVal}.
+
+Arguments Exists {nVal}.
+
+Arguments Or {nVal}.
+
+Arguments Fail {nVal}.
+
+Arguments One {nVal}.
+
+Arguments All {nVal}.
+
+Arguments SCchoicehole {nVal}.
+
+Arguments SCchoiceleft {nVal}.
+
+Arguments SCchoiceright {nVal}.
+
+Arguments SXone {nVal}.
+
+Arguments SXall {nVal}.
+
+Arguments EHole {nVal}.
+
+Arguments ESeq1 {nVal}.
+
+Arguments ESeq2 {nVal}.
+
+Arguments EUnify1 {nVal}.
+
+Arguments EUnify2 {nVal}.
+
+Arguments EExists {nVal}.
+
+Arguments EOr1 {nVal}.
+
+Arguments EOr2 {nVal}.
+
+Arguments EOne {nVal}.
+
+Arguments EAll {nVal}.
+
+Arguments EApp1 {nVal}.
+
+Arguments EApp2 {nVal}.
+
+Arguments ERet {nVal}.
+
+Arguments VTuple {nVal}.
+
+Arguments VLam {nVal}.
+
+Arguments VEcons1 {nVal}.
+
+Arguments VEcons2 {nVal}.
+
+Arguments CXhole {nVal}.
+
+Arguments CXchoiceright {nVal}.
+
+Arguments CXseqleft {nVal}.
+
+Arguments CXseqright {nVal}.
+
+Arguments CXexists {nVal}.
+
+Arguments Xhole {nVal}.
+
+Arguments Xeqright {nVal}.
+
+Arguments Xseqleft {nVal}.
+
+Arguments Xseqright {nVal}.
+
+Global Instance Subst_Val { mVal : nat } { nVal : nat } : Subst1 ((fin) (mVal) -> Val (nVal)) (Val (mVal)) (Val (nVal)) := @subst_Val (mVal) (nVal) .
+
+Global Instance Subst_Exp { mVal : nat } { nVal : nat } : Subst1 ((fin) (mVal) -> Val (nVal)) (Exp (mVal)) (Exp (nVal)) := @subst_Exp (mVal) (nVal) .
+
+Global Instance Subst_SC { mVal : nat } { nVal : nat } : Subst1 ((fin) (mVal) -> Val (nVal)) (SC (mVal)) (SC (nVal)) := @subst_SC (mVal) (nVal) .
+
+Global Instance Subst_scopeContext { mVal : nat } { nVal : nat } : Subst1 ((fin) (mVal) -> Val (nVal)) (scopeContext (mVal)) (scopeContext (nVal)) := @subst_scopeContext (mVal) (nVal) .
+
+Global Instance Subst_ExpCompatContext { mVal : nat } { nVal : nat } : Subst1 ((fin) (mVal) -> Val (nVal)) (ExpCompatContext (mVal)) (ExpCompatContext (nVal)) := @subst_ExpCompatContext (mVal) (nVal) .
+
+Global Instance Subst_ValCompatContext { mVal : nat } { nVal : nat } : Subst1 ((fin) (mVal) -> Val (nVal)) (ValCompatContext (mVal)) (ValCompatContext (nVal)) := @subst_ValCompatContext (mVal) (nVal) .
+
+Global Instance Subst_ValListCompatContext { mVal : nat } { nVal : nat } : Subst1 ((fin) (mVal) -> Val (nVal)) (ValListCompatContext (mVal)) (ValListCompatContext (nVal)) := @subst_ValListCompatContext (mVal) (nVal) .
+
+Global Instance Subst_choiceContext { mVal : nat } { nVal : nat } : Subst1 ((fin) (mVal) -> Val (nVal)) (choiceContext (mVal)) (choiceContext (nVal)) := @subst_choiceContext (mVal) (nVal) .
+
+Global Instance Subst_exContext { mVal : nat } { nVal : nat } : Subst1 ((fin) (mVal) -> Val (nVal)) (exContext (mVal)) (exContext (nVal)) := @subst_exContext (mVal) (nVal) .
+
+Global Instance Ren_Val { mVal : nat } { nVal : nat } : Ren1 ((fin) (mVal) -> (fin) (nVal)) (Val (mVal)) (Val (nVal)) := @ren_Val (mVal) (nVal) .
+
+Global Instance Ren_Exp { mVal : nat } { nVal : nat } : Ren1 ((fin) (mVal) -> (fin) (nVal)) (Exp (mVal)) (Exp (nVal)) := @ren_Exp (mVal) (nVal) .
+
+(*
+Global Instance Ren_SC { mVal : nat } { nVal : nat } : Ren1 ((fin) (mVal) -> (fin) (nVal)) (SC (mVal)) (SC (nVal)) := @ren_SC (mVal) (nVal) .
+
+Global Instance Ren_scopeContext { mVal : nat } { nVal : nat } : Ren1 ((fin) (mVal) -> (fin) (nVal)) (scopeContext (mVal)) (scopeContext (nVal)) := @ren_scopeContext (mVal) (nVal) .
+
+Global Instance Ren_ExpCompatContext { mVal : nat } { nVal : nat } : Ren1 ((fin) (mVal) -> (fin) (nVal)) (ExpCompatContext (mVal)) (ExpCompatContext (nVal)) := @ren_ExpCompatContext (mVal) (nVal) .
+
+Global Instance Ren_ValCompatContext { mVal : nat } { nVal : nat } : Ren1 ((fin) (mVal) -> (fin) (nVal)) (ValCompatContext (mVal)) (ValCompatContext (nVal)) := @ren_ValCompatContext (mVal) (nVal) .
+
+Global Instance Ren_ValListCompatContext { mVal : nat } { nVal : nat } : Ren1 ((fin) (mVal) -> (fin) (nVal)) (ValListCompatContext (mVal)) (ValListCompatContext (nVal)) := @ren_ValListCompatContext (mVal) (nVal) .
+
+Global Instance Ren_choiceContext { mVal : nat } { nVal : nat } : Ren1 ((fin) (mVal) -> (fin) (nVal)) (choiceContext (mVal)) (choiceContext (nVal)) := @ren_choiceContext (mVal) (nVal) .
+
+Global Instance Ren_exContext { mVal : nat } { nVal : nat } : Ren1 ((fin) (mVal) -> (fin) (nVal)) (exContext (mVal)) (exContext (nVal)) := @ren_exContext (mVal) (nVal) .
+*)
+
+Global Instance VarInstance_Val { mVal : nat } : Var ((fin) (mVal)) (Val (mVal)) := @var_Val (mVal) .
 
 Notation "x '__Val'" := (var_Val x) (at level 5, format "x __Val") : subst_scope.
 
@@ -524,9 +990,13 @@ Notation "x '__Val'" := (@ids (_) (_) VarInstance_Val x) (at level 5, only print
 
 Notation "'var'" := (var_Val) (only printing, at level 1) : subst_scope.
 
+Class Up_Val X Y := up_Val : X -> Y.
+
 Notation "↑__Val" := (up_Val) (only printing) : subst_scope.
 
 Notation "↑__Val" := (up_Val_Val) (only printing) : subst_scope.
+
+Global Instance Up_Val_Val { m : nat } { nVal : nat } : Up_Val (_) (_) := @up_Val_Val (m) (nVal) .
 
 Notation "s [ sigmaVal ]" := (subst_Val sigmaVal s) (at level 7, left associativity, only printing) : subst_scope.
 
@@ -544,14 +1014,39 @@ Notation "s ⟨ xiVal ⟩" := (ren_Exp xiVal s) (at level 7, left associativity,
 
 Notation "⟨ xiVal ⟩" := (ren_Exp xiVal) (at level 1, left associativity, only printing) : fscope.
 
-End SubstNotations.
+Notation "s [ sigmaVal ]" := (subst_SC sigmaVal s) (at level 7, left associativity, only printing) : subst_scope.
 
+Notation "[ sigmaVal ]" := (subst_SC sigmaVal) (at level 1, left associativity, only printing) : fscope.
 
-Ltac auto_unfold := repeat unfold subst1,  subst2,  Subst1,  Subst2,  ids,  ren1,  ren2,  Ren1,  Ren2,  Subst_Val,  Subst_Exp,  Ren_Val,  Ren_Exp,  VarInstance_Val.
+Notation "s [ sigmaVal ]" := (subst_scopeContext sigmaVal s) (at level 7, left associativity, only printing) : subst_scope.
 
-Tactic Notation "auto_unfold" "in" "*" := repeat unfold subst1,  subst2,  Subst1,  Subst2,  ids,  ren1,  ren2,  Ren1,  Ren2,  Subst_Val,  Subst_Exp,  Ren_Val,  Ren_Exp,  VarInstance_Val in *.
+Notation "[ sigmaVal ]" := (subst_scopeContext sigmaVal) (at level 1, left associativity, only printing) : fscope.
 
-Ltac asimpl' := repeat first [progress rewrite ?instId_Val| progress rewrite ?compComp_Val| progress rewrite ?compComp'_Val| progress rewrite ?instId_Exp| progress rewrite ?compComp_Exp| progress rewrite ?compComp'_Exp| progress rewrite ?rinstId_Val| progress rewrite ?compRen_Val| progress rewrite ?compRen'_Val| progress rewrite ?renComp_Val| progress rewrite ?renComp'_Val| progress rewrite ?renRen_Val| progress rewrite ?renRen'_Val| progress rewrite ?rinstId_Exp| progress rewrite ?compRen_Exp| progress rewrite ?compRen'_Exp| progress rewrite ?renComp_Exp| progress rewrite ?renComp'_Exp| progress rewrite ?renRen_Exp| progress rewrite ?renRen'_Exp| progress rewrite ?varL_Val| progress rewrite ?varLRen_Val| progress (unfold up_ren, upRen_Val_Val, up_Val_Val)| progress (cbn [subst_Val subst_Exp ren_Val ren_Exp])| fsimpl].
+Notation "s [ sigmaVal ]" := (subst_ExpCompatContext sigmaVal s) (at level 7, left associativity, only printing) : subst_scope.
+
+Notation "[ sigmaVal ]" := (subst_ExpCompatContext sigmaVal) (at level 1, left associativity, only printing) : fscope.
+
+Notation "s [ sigmaVal ]" := (subst_ValCompatContext sigmaVal s) (at level 7, left associativity, only printing) : subst_scope.
+
+Notation "[ sigmaVal ]" := (subst_ValCompatContext sigmaVal) (at level 1, left associativity, only printing) : fscope.
+
+Notation "s [ sigmaVal ]" := (subst_ValListCompatContext sigmaVal s) (at level 7, left associativity, only printing) : subst_scope.
+
+Notation "[ sigmaVal ]" := (subst_ValListCompatContext sigmaVal) (at level 1, left associativity, only printing) : fscope.
+
+Notation "s [ sigmaVal ]" := (subst_choiceContext sigmaVal s) (at level 7, left associativity, only printing) : subst_scope.
+
+Notation "[ sigmaVal ]" := (subst_choiceContext sigmaVal) (at level 1, left associativity, only printing) : fscope.
+
+Notation "s [ sigmaVal ]" := (subst_exContext sigmaVal s) (at level 7, left associativity, only printing) : subst_scope.
+
+Notation "[ sigmaVal ]" := (subst_exContext sigmaVal) (at level 1, left associativity, only printing) : fscope.
+
+Ltac auto_unfold := repeat unfold subst1,  subst2,  Subst1,  Subst2,  ids,  ren1,  ren2,  Ren1,  Ren2,  Subst_Val,  Subst_Exp,  Subst_SC,  Subst_scopeContext,  Subst_ExpCompatContext,  Subst_ValCompatContext,  Subst_ValListCompatContext,  Subst_choiceContext,  Subst_exContext,  Ren_Val,  Ren_Exp,  VarInstance_Val.
+
+Tactic Notation "auto_unfold" "in" "*" := repeat unfold subst1,  subst2,  Subst1,  Subst2,  ids,  ren1,  ren2,  Ren1,  Ren2,  Subst_Val,  Subst_Exp,  Subst_SC,  Subst_scopeContext,  Subst_ExpCompatContext,  Subst_ValCompatContext,  Subst_ValListCompatContext,  Subst_choiceContext,  Subst_exContext,  Ren_Val,  Ren_Exp,  VarInstance_Val in *.
+
+Ltac asimpl' := repeat first [progress rewrite ?instId_Val| progress rewrite ?compComp_Val| progress rewrite ?compComp'_Val| progress rewrite ?instId_Exp| progress rewrite ?compComp_Exp| progress rewrite ?compComp'_Exp| progress rewrite ?instId_SC| progress rewrite ?compComp_SC| progress rewrite ?compComp'_SC| progress rewrite ?instId_scopeContext| progress rewrite ?compComp_scopeContext| progress rewrite ?compComp'_scopeContext| progress rewrite ?instId_ExpCompatContext| progress rewrite ?compComp_ExpCompatContext| progress rewrite ?compComp'_ExpCompatContext| progress rewrite ?instId_ValCompatContext| progress rewrite ?compComp_ValCompatContext| progress rewrite ?compComp'_ValCompatContext| progress rewrite ?instId_ValListCompatContext| progress rewrite ?compComp_ValListCompatContext| progress rewrite ?compComp'_ValListCompatContext| progress rewrite ?instId_choiceContext| progress rewrite ?compComp_choiceContext| progress rewrite ?compComp'_choiceContext| progress rewrite ?instId_exContext| progress rewrite ?compComp_exContext| progress rewrite ?compComp'_exContext| progress rewrite ?rinstId_Val| progress rewrite ?compRen_Val| progress rewrite ?compRen'_Val| progress rewrite ?renComp_Val| progress rewrite ?renComp'_Val| progress rewrite ?renRen_Val| progress rewrite ?renRen'_Val| progress rewrite ?rinstId_Exp| progress rewrite ?compRen_Exp| progress rewrite ?compRen'_Exp| progress rewrite ?renComp_Exp| progress rewrite ?renComp'_Exp| progress rewrite ?renRen_Exp| progress rewrite ?renRen'_Exp| progress rewrite ?varL_Val| progress rewrite ?varLRen_Val| progress (unfold up_ren, upRen_Val_Val, up_Val_Val)| progress (cbn [subst_Val subst_Exp subst_SC subst_scopeContext subst_ExpCompatContext subst_ValCompatContext subst_ValListCompatContext subst_choiceContext subst_exContext ren_Val ren_Exp])| fsimpl].
 
 Ltac asimpl := repeat try unfold_funcomp; auto_unfold in *; asimpl'; repeat try unfold_funcomp.
 
@@ -559,7 +1054,7 @@ Tactic Notation "asimpl" "in" hyp(J) := revert J; asimpl; intros J.
 
 Tactic Notation "auto_case" := auto_case (asimpl; cbn; eauto).
 
-Tactic Notation "asimpl" "in" "*" := auto_unfold in *; repeat first [progress rewrite ?instId_Val in *| progress rewrite ?compComp_Val in *| progress rewrite ?compComp'_Val in *| progress rewrite ?instId_Exp in *| progress rewrite ?compComp_Exp in *| progress rewrite ?compComp'_Exp in *| progress rewrite ?rinstId_Val in *| progress rewrite ?compRen_Val in *| progress rewrite ?compRen'_Val in *| progress rewrite ?renComp_Val in *| progress rewrite ?renComp'_Val in *| progress rewrite ?renRen_Val in *| progress rewrite ?renRen'_Val in *| progress rewrite ?rinstId_Exp in *| progress rewrite ?compRen_Exp in *| progress rewrite ?compRen'_Exp in *| progress rewrite ?renComp_Exp in *| progress rewrite ?renComp'_Exp in *| progress rewrite ?renRen_Exp in *| progress rewrite ?renRen'_Exp in *| progress rewrite ?varL_Val in *| progress rewrite ?varLRen_Val in *| progress (unfold up_ren, upRen_Val_Val, up_Val_Val in *)| progress (cbn [subst_Val subst_Exp ren_Val ren_Exp] in *)| fsimpl in *].
+Tactic Notation "asimpl" "in" "*" := auto_unfold in *; repeat first [progress rewrite ?instId_Val in *| progress rewrite ?compComp_Val in *| progress rewrite ?compComp'_Val in *| progress rewrite ?instId_Exp in *| progress rewrite ?compComp_Exp in *| progress rewrite ?compComp'_Exp in *| progress rewrite ?instId_SC in *| progress rewrite ?compComp_SC in *| progress rewrite ?compComp'_SC in *| progress rewrite ?instId_scopeContext in *| progress rewrite ?compComp_scopeContext in *| progress rewrite ?compComp'_scopeContext in *| progress rewrite ?instId_ExpCompatContext in *| progress rewrite ?compComp_ExpCompatContext in *| progress rewrite ?compComp'_ExpCompatContext in *| progress rewrite ?instId_ValCompatContext in *| progress rewrite ?compComp_ValCompatContext in *| progress rewrite ?compComp'_ValCompatContext in *| progress rewrite ?instId_ValListCompatContext in *| progress rewrite ?compComp_ValListCompatContext in *| progress rewrite ?compComp'_ValListCompatContext in *| progress rewrite ?instId_choiceContext in *| progress rewrite ?compComp_choiceContext in *| progress rewrite ?compComp'_choiceContext in *| progress rewrite ?instId_exContext in *| progress rewrite ?compComp_exContext in *| progress rewrite ?compComp'_exContext in *| progress rewrite ?rinstId_Val in *| progress rewrite ?compRen_Val in *| progress rewrite ?compRen'_Val in *| progress rewrite ?renComp_Val in *| progress rewrite ?renComp'_Val in *| progress rewrite ?renRen_Val in *| progress rewrite ?renRen'_Val in *| progress rewrite ?rinstId_Exp in *| progress rewrite ?compRen_Exp in *| progress rewrite ?compRen'_Exp in *| progress rewrite ?renComp_Exp in *| progress rewrite ?renComp'_Exp in *| progress rewrite ?renRen_Exp in *| progress rewrite ?renRen'_Exp in *| progress rewrite ?varL_Val in *| progress rewrite ?varLRen_Val in *| progress (unfold up_ren, upRen_Val_Val, up_Val_Val in *)| progress (cbn [subst_Val subst_Exp subst_SC subst_scopeContext subst_ExpCompatContext subst_ValCompatContext subst_ValListCompatContext subst_choiceContext subst_exContext ren_Val ren_Exp] in *)| fsimpl in *].
 
 Ltac substify := auto_unfold; try repeat (erewrite rinstInst_Val); try repeat (erewrite rinstInst_Exp).
 
